src/MessagePool.v
@@ -5,617 +5,694 @@ Set Implicit Arguments.
 
 Section MessagePool.
   Variable (MsgT: Type).
-  Context `{HasMsg MsgT}.
 
   Definition Queue := list MsgT.
-  Definition MessagePool := list MsgT.
+  Definition MessagePool := M.t (list MsgT).
 
-  Definition isAddrOf (from to chn: IdxT) (msg: MsgT) :=
-    if msgAddr_dec (mid_addr (msg_id (getMsg msg))) (buildMsgAddr from to chn)
-    then true
-    else false.
+  Definition emptyMP: MessagePool := M.empty _.
 
-  Definition findMP (from to chn: IdxT) (mp: MessagePool): Queue :=
-    filter (fun msg => isAddrOf from to chn msg) mp.
+  Definition findQ (midx: IdxT) (mp: MessagePool): Queue :=
+    mp@[midx] >>=[nil] (fun q => q).
 
-  Definition firstMP (from to chn: IdxT) (mp: MessagePool) :=
-    hd_error (findMP from to chn mp).
+  Definition firstMP (midx: IdxT) (mp: MessagePool) :=
+    hd_error (findQ midx mp).
 
-  Fixpoint firstMP' (from to chn: IdxT) (mp: MessagePool) :=
-    match mp with
-    | nil => None
-    | msg :: mp' =>
-      if isAddrOf from to chn msg
-      then Some msg
-      else firstMP' from to chn mp'
-    end.
+  Definition FirstMP (midx: IdxT) (msg: MsgT) (mp: MessagePool) :=
+    firstMP midx mp = Some msg.
 
-  Fixpoint deqMP (from to chn: IdxT) (mp: MessagePool): MessagePool :=
-    match mp with
-    | nil => nil
-    | msg :: mp' =>
-      if isAddrOf from to chn msg
-      then mp'
-      else msg :: deqMP from to chn mp'
+  (* NOTE: the head is the oldest one. *)
+  Definition deqMP (midx: IdxT) (mp: MessagePool): MessagePool :=
+    match findQ midx mp with
+    | nil => mp
+    | _ :: q => mp+[midx <- q]
     end.
 
   (* NOTE: the head is the oldest one. *)
-  Definition enqMP (m: MsgT) (mp: MessagePool): MessagePool := mp ++ (m :: nil).
+  Definition enqMP (midx: IdxT) (m: MsgT) (mp: MessagePool): MessagePool :=
+    mp+[midx <- (match findQ midx mp with
+                 | nil => [m]
+                 | q => q ++ [m]
+                 end)].
 
-  Definition removeMP (m: MsgT) (mp: MessagePool): MessagePool :=
-    let mid := msg_id (getMsg m) in
-    deqMP (mid_from mid) (mid_to mid) (mid_chn mid) mp.
-
-  Definition FirstMP (mp: MessagePool) (m: MsgT) :=
-    let mid := msg_id (getMsg m) in
-    firstMP (mid_from mid) (mid_to mid) (mid_chn mid) mp = Some m.
-  
-  Definition EmptyMP (mp: MessagePool) := mp = nil.
-  Definition InMP (msg: MsgT) (mp: MessagePool) := In msg mp.
+  Definition EmptyMP (mp: MessagePool) := mp = M.empty _.
+  Definition InMP (midx: IdxT) (msg: MsgT) (mp: MessagePool) :=
+    In msg (findQ midx mp).
 
   Definition ForallMP (P: MsgT -> Prop) (mp: MessagePool) :=
-    Forall P mp.
+    forall midx, Forall P (findQ midx mp).
 
-  Definition distributeMsgs (nmsgs: list MsgT) (mp: MessagePool): MessagePool :=
-    mp ++ nmsgs.
-
-  Fixpoint removeMsgs (dmsgs: list MsgT) (mp: MessagePool): MessagePool :=
-    match dmsgs with
+  Fixpoint enqMsgs (nmsgs: list (Id MsgT)) (mp: MessagePool): MessagePool :=
+    match nmsgs with
     | nil => mp
-    | dmsg :: dmsgs' =>
-      removeMsgs dmsgs' (removeMP dmsg mp)
+    | (midx, msg) :: nmsgs' =>
+      enqMsgs nmsgs' (enqMP midx msg mp)
+    end.
+
+  Fixpoint deqMsgs (minds: list IdxT) (mp: MessagePool): MessagePool :=
+    match minds with
+    | nil => mp
+    | mind :: minds' =>
+      deqMsgs minds' (deqMP mind mp)
     end.
 
 End MessagePool.
 
 Section Facts.
   Variable (MsgT: Type).
-  Context `{HasMsg MsgT}.
-
-  Lemma firstMP_firstMP':
-    forall from to chn mp,
-      firstMP from to chn mp = firstMP' from to chn mp.
-  Proof.
-    induction mp; simpl; intros; [reflexivity|].
-    unfold firstMP, findMP; simpl.
-    destruct (isAddrOf _ _ _ _); auto.
-  Qed.
-
-  Lemma firstMP_app_or:
-    forall (msg: MsgT) from to chn mp1 mp2,
-      firstMP from to chn (mp1 ++ mp2) = Some msg ->
-      firstMP from to chn mp1 = Some msg \/
-      firstMP from to chn mp2 = Some msg.
-  Proof.
-    induction mp1; intros; auto.
-    unfold firstMP in *; simpl in *.
-    destruct (isAddrOf _ _ _ _).
-    - left; inv H0; reflexivity.
-    - auto.
-  Qed.
-
-  Lemma firstMP_enqMP_or:
-    forall (msg nmsg: MsgT) from to chn mp,
-      firstMP from to chn (enqMP nmsg mp) = Some msg ->
-      msg = nmsg \/ firstMP from to chn mp = Some msg.
-  Proof.
-    intros.
-    apply firstMP_app_or in H0; destruct H0; auto.
-    unfold firstMP in H0; cbn in H0.
-    destruct (isAddrOf _ _ _ _); [|discriminate].
-    inv H0; auto.
-  Qed.
-
-  Lemma firstMP_distributeMsgs_or:
-    forall (msg: MsgT) from to chn nmsgs mp,
-      firstMP from to chn (distributeMsgs nmsgs mp) = Some msg ->
-      firstMP from to chn mp = Some msg \/
-      firstMP from to chn nmsgs = Some msg.
-  Proof.
-    intros.
-    apply firstMP_app_or; auto.
-  Qed.
-
-  Lemma inMP_enqMP_or:
-    forall (msg: MsgT) nmsg mp,
-      InMP msg (enqMP nmsg mp) ->
-      msg = nmsg \/ InMP msg mp.
-  Proof.
-    intros.
-    apply in_app_or in H0; destruct H0; auto.
-    Common.dest_in; auto.
-  Qed.
-
-  Lemma inMP_deqMP:
-    forall (msg: MsgT) from to chn mp,
-      InMP msg (deqMP from to chn mp) ->
-      InMP msg mp.
-  Proof.
-    induction mp; simpl; intros; auto.
-    find_if_inside; auto.
-    inv H0; auto.
-  Qed.
-
-  Lemma inMP_distributeMsgs_or:
-    forall (msg: MsgT) nmsgs mp,
-      InMP msg (distributeMsgs nmsgs mp) ->
-      In msg nmsgs \/ InMP msg mp.
-  Proof.
-    intros; apply in_app_or in H0; destruct H0; auto.
-  Qed.
-
-  Lemma firstMP_InMP:
-    forall (msg: MsgT) from to chn mp,
-      firstMP from to chn mp = Some msg ->
-      InMP msg mp.
-  Proof.
-    induction mp; simpl; intros; [discriminate|].
-    unfold firstMP in H0; simpl in H0.
-    destruct (isAddrOf _ _ _ _).
-    - inv H0; auto.
-    - right; apply IHmp; auto.
-  Qed.
-
-  Lemma FirstMP_InMP:
-    forall (msg: MsgT) mp,
-      FirstMP mp msg ->
-      InMP msg mp.
-  Proof.
-    unfold FirstMP; intros.
-    eapply firstMP_InMP; eauto.
-  Qed.
-
-  Lemma ForallMP_InMP_SubList:
-    forall (msgs: list MsgT) mp,
-      ForallMP (fun msg => InMP msg mp) msgs ->
-      SubList msgs mp.
-  Proof.
-    induction msgs; intros; [apply SubList_nil|].
-    inv H0.
-    apply SubList_cons; auto.
-  Qed.
-
-  Lemma InMP_deqMP:
-    forall msg from to chn mp,
-      InMP msg (deqMP from to chn mp) ->
-      InMP msg mp.
-  Proof.
-    induction mp; simpl; intros; auto.
-    destruct (isAddrOf _ _ _ _); auto.
-    inv H0; auto.
-  Qed.
-
-  Lemma InMP_removeMP:
-    forall msg rmsg mp,
-      InMP msg (removeMP rmsg mp) ->
-      InMP msg mp.
-  Proof.
-    unfold removeMP; intros.
-    eapply InMP_deqMP; eauto.
-  Qed.
-
-  Lemma InMP_removeMsgs:
-    forall msg rmsgs mp,
-      InMP msg (removeMsgs rmsgs mp) ->
-      InMP msg mp.
-  Proof.
-    induction rmsgs; simpl; intros; auto.
-    eapply InMP_removeMP; eauto.
-  Qed.
-
-  Lemma ForallMP_forall:
-    forall P mp,
-      ForallMP P mp <->
-      (forall msg: MsgT, InMP msg mp -> P msg).
-  Proof.
-    intros; apply Forall_forall.
-  Qed.
-
-  Lemma ForallMP_SubList:
-    forall P (mp1 mp2: MessagePool MsgT),
-      ForallMP P mp2 ->
-      SubList mp1 mp2 ->
-      ForallMP P mp1.
-  Proof.
-    intros.
-    apply ForallMP_forall; intros.
-    eapply ForallMP_forall in H0; eauto.
-    apply H1; auto.
-  Qed.
 
   Lemma ForallMP_enqMP:
-    forall (P: MsgT -> Prop) (msg: MsgT) mp,
+    forall P (mp: MessagePool MsgT),
       ForallMP P mp ->
-      P msg ->
-      ForallMP P (enqMP msg mp).
+      forall i m,
+        P m ->
+        ForallMP P (enqMP i m mp).
   Proof.
-    intros.
-    apply Forall_app; auto.
+    unfold ForallMP, enqMP, findQ; intros.
+    remember (mp@[i]) as iq; destruct iq; simpl.
+    - findeq; auto.
+      specialize (H i).
+      mred_find.
+      destruct l; simpl; auto.
+      inv H.
+      constructor; auto.
+      apply Forall_app; auto.
+    - findeq; simpl; auto.
+  Qed.
+
+  Lemma ForallMP_enqMsgs:
+    forall P nmsgs (mp: MessagePool MsgT),
+      ForallMP P mp ->
+      Forall P (valsOf nmsgs) ->
+      ForallMP P (enqMsgs nmsgs mp).
+  Proof.
+    induction nmsgs; simpl; intros; auto.
+    destruct a as [i m]; cbn in *.
+    inv H0.
+    apply IHnmsgs; auto.
+    apply ForallMP_enqMP; auto.
   Qed.
 
   Lemma ForallMP_deqMP:
-    forall (P: MsgT -> Prop) from to chn mp,
+    forall P (mp: MessagePool MsgT),
       ForallMP P mp ->
-      ForallMP P (deqMP from to chn mp).
+      forall i,
+        ForallMP P (deqMP i mp).
   Proof.
-    induction mp; simpl; intros; auto.
-    inv H0.
-    find_if_inside; auto.
-    constructor; auto.
-    apply IHmp; auto.
+    unfold ForallMP, deqMP, findQ; intros.
+    remember (mp@[i]) as iq; destruct iq; simpl.
+    - destruct l; auto.
+      findeq; auto; simpl.
+      specialize (H i); mred_find.
+      inv H; auto.
+    - findeq; simpl; auto.
   Qed.
 
-  Lemma ForallMP_removeMP:
-    forall (P: MsgT -> Prop) msg mp,
+  Lemma ForallMP_deqMsgs:
+    forall P minds (mp: MessagePool MsgT),
       ForallMP P mp ->
-      ForallMP P (removeMP msg mp).
+      ForallMP P (deqMsgs minds mp).
   Proof.
-    induction mp; simpl; intros; auto.
-    inv H0.
-    cbn; destruct (isAddrOf _ _ _ _); auto.
-    constructor; auto.
+    induction minds; simpl; intros; auto.
+    apply IHminds; auto.
     apply ForallMP_deqMP; auto.
   Qed.
 
-  Lemma ForallMP_distributeMsgs:
-    forall (P: MsgT -> Prop) (nmsgs: list MsgT) mp,
-      ForallMP P mp ->
-      ForallMP P nmsgs ->
-      ForallMP P (distributeMsgs nmsgs mp).
+  Lemma ForallMP_impl:
+    forall (P1: MsgT -> Prop) mp,
+      ForallMP P1 mp ->
+      forall (P2: MsgT -> Prop),
+        (forall m, P1 m -> P2 m) ->
+        ForallMP P2 mp.
   Proof.
-    intros.
-    apply Forall_app; auto.
-  Qed.
+  Admitted.
 
-  Lemma ForallMP_removeMsgs:
-    forall (P: MsgT -> Prop) (dmsgs: list MsgT) mp,
+  Lemma ForallMP_InMP:
+    forall (P: MsgT -> Prop) mp,
       ForallMP P mp ->
-      ForallMP P (removeMsgs dmsgs mp).
+      forall i m,
+        InMP i m mp ->
+        P m.
   Proof.
-    induction dmsgs; simpl; intros; auto.
-    apply IHdmsgs.
-    apply ForallMP_removeMP; auto.
-  Qed.
+  Admitted.
 
-  Lemma ForallMP_removeOnce:
-    forall (msg_dec: forall m1 m2: MsgT, {m1 = m2} + {m1 <> m2})
-           (P: MsgT -> Prop) tmsg mp,
+  Corollary ForallMP_Forall_InMP:
+    forall (P: MsgT -> Prop) mp,
       ForallMP P mp ->
-      ForallMP P (removeOnce msg_dec tmsg mp).
+      forall ims,
+        Forall (fun im => InMP (idOf im) (valOf im) mp) ims ->
+        Forall P (valsOf ims).
   Proof.
-    induction mp; simpl; intros; auto.
+    induction ims; simpl; intros; auto.
     inv H0.
-    find_if_inside; auto.
     constructor; auto.
-    apply IHmp; auto.
+    eapply ForallMP_InMP; eauto.
   Qed.
+
+  Lemma FirstMP_InMP:
+    forall (mp: MessagePool MsgT) i m,
+      FirstMP i m mp ->
+      InMP i m mp.
+  Proof.
+  Admitted.
+
+  (* Lemma firstMP_app_or: *)
+  (*   forall (msg: MsgT) mind mp1 mp2, *)
+  (*     firstMP mind (mp1 ++ mp2) = Some msg -> *)
+  (*     firstMP mind mp1 = Some msg \/ *)
+  (*     firstMP mind mp2 = Some msg. *)
+  (* Proof. *)
+  (*   induction mp1; intros; auto. *)
+  (*   unfold firstMP in *; simpl in *. *)
+  (*   destruct (isAddrOf _ _ _ _). *)
+  (*   - left; inv H0; reflexivity. *)
+  (*   - auto. *)
+  (* Qed. *)
+
+  (* Lemma firstMP_enqMP_or: *)
+  (*   forall (msg nmsg: MsgT) mind mp, *)
+  (*     firstMP mind (enqMP nmsg mp) = Some msg -> *)
+  (*     msg = nmsg \/ firstMP mind mp = Some msg. *)
+  (* Proof. *)
+  (*   intros. *)
+  (*   apply firstMP_app_or in H0; destruct H0; auto. *)
+  (*   unfold firstMP in H0; cbn in H0. *)
+  (*   destruct (isAddrOf _ _ _ _); [|discriminate]. *)
+  (*   inv H0; auto. *)
+  (* Qed. *)
+
+  (* Lemma firstMP_enqMsgs_or: *)
+  (*   forall (msg: MsgT) mind nmsgs mp, *)
+  (*     firstMP mind (enqMsgs nmsgs mp) = Some msg -> *)
+  (*     firstMP mind mp = Some msg \/ *)
+  (*     firstMP mind nmsgs = Some msg. *)
+  (* Proof. *)
+  (*   intros. *)
+  (*   apply firstMP_app_or; auto. *)
+  (* Qed. *)
+
+  (* Lemma inMP_enqMP_or: *)
+  (*   forall (msg: MsgT) nmsg mp, *)
+  (*     InMP msg (enqMP nmsg mp) -> *)
+  (*     msg = nmsg \/ InMP msg mp. *)
+  (* Proof. *)
+  (*   intros. *)
+  (*   apply in_app_or in H0; destruct H0; auto. *)
+  (*   Common.dest_in; auto. *)
+  (* Qed. *)
+
+  (* Lemma inMP_deqMP: *)
+  (*   forall (msg: MsgT) mind mp, *)
+  (*     InMP msg (deqMP mind mp) -> *)
+  (*     InMP msg mp. *)
+  (* Proof. *)
+  (*   induction mp; simpl; intros; auto. *)
+  (*   find_if_inside; auto. *)
+  (*   inv H0; auto. *)
+  (* Qed. *)
+
+  (* Lemma inMP_enqMsgs_or: *)
+  (*   forall (msg: MsgT) nmsgs mp, *)
+  (*     InMP msg (enqMsgs nmsgs mp) -> *)
+  (*     In msg nmsgs \/ InMP msg mp. *)
+  (* Proof. *)
+  (*   intros; apply in_app_or in H0; destruct H0; auto. *)
+  (* Qed. *)
+
+  (* Lemma firstMP_InMP: *)
+  (*   forall (msg: MsgT) mind mp, *)
+  (*     firstMP mind mp = Some msg -> *)
+  (*     InMP msg mp. *)
+  (* Proof. *)
+  (*   induction mp; simpl; intros; [discriminate|]. *)
+  (*   unfold firstMP in H0; simpl in H0. *)
+  (*   destruct (isAddrOf _ _ _ _). *)
+  (*   - inv H0; auto. *)
+  (*   - right; apply IHmp; auto. *)
+  (* Qed. *)
+
+  (* Lemma FirstMP_InMP: *)
+  (*   forall (msg: MsgT) mp, *)
+  (*     FirstMP mp msg -> *)
+  (*     InMP msg mp. *)
+  (* Proof. *)
+  (*   unfold FirstMP; intros. *)
+  (*   eapply firstMP_InMP; eauto. *)
+  (* Qed. *)
+
+  (* Lemma ForallMP_InMP_SubList: *)
+  (*   forall (msgs: list MsgT) mp, *)
+  (*     ForallMP (fun msg => InMP msg mp) msgs -> *)
+  (*     SubList msgs mp. *)
+  (* Proof. *)
+  (*   induction msgs; intros; [apply SubList_nil|]. *)
+  (*   inv H0. *)
+  (*   apply SubList_cons; auto. *)
+  (* Qed. *)
+
+  (* Lemma InMP_deqMP: *)
+  (*   forall msg mind mp, *)
+  (*     InMP msg (deqMP mind mp) -> *)
+  (*     InMP msg mp. *)
+  (* Proof. *)
+  (*   induction mp; simpl; intros; auto. *)
+  (*   destruct (isAddrOf _ _ _ _); auto. *)
+  (*   inv H0; auto. *)
+  (* Qed. *)
+
+  (* Lemma InMP_removeMP: *)
+  (*   forall msg rmsg mp, *)
+  (*     InMP msg (removeMP rmsg mp) -> *)
+  (*     InMP msg mp. *)
+  (* Proof. *)
+  (*   unfold removeMP; intros. *)
+  (*   eapply InMP_deqMP; eauto. *)
+  (* Qed. *)
+
+  (* Lemma InMP_deqMsgs: *)
+  (*   forall msg rmsgs mp, *)
+  (*     InMP msg (deqMsgs rmsgs mp) -> *)
+  (*     InMP msg mp. *)
+  (* Proof. *)
+  (*   induction rmsgs; simpl; intros; auto. *)
+  (*   eapply InMP_removeMP; eauto. *)
+  (* Qed. *)
+
+  (* Lemma ForallMP_forall: *)
+  (*   forall P mp, *)
+  (*     ForallMP P mp <-> *)
+  (*     (forall msg: MsgT, InMP msg mp -> P msg). *)
+  (* Proof. *)
+  (*   intros; apply Forall_forall. *)
+  (* Qed. *)
+
+  (* Lemma ForallMP_SubList: *)
+  (*   forall P (mp1 mp2: MessagePool MsgT), *)
+  (*     ForallMP P mp2 -> *)
+  (*     SubList mp1 mp2 -> *)
+  (*     ForallMP P mp1. *)
+  (* Proof. *)
+  (*   intros. *)
+  (*   apply ForallMP_forall; intros. *)
+  (*   eapply ForallMP_forall in H0; eauto. *)
+  (*   apply H1; auto. *)
+  (* Qed. *)
+
+  (* Lemma ForallMP_enqMP: *)
+  (*   forall (P: MsgT -> Prop) (msg: MsgT) mp, *)
+  (*     ForallMP P mp -> *)
+  (*     P msg -> *)
+  (*     ForallMP P (enqMP msg mp). *)
+  (* Proof. *)
+  (*   intros. *)
+  (*   apply Forall_app; auto. *)
+  (* Qed. *)
+
+  (* Lemma ForallMP_deqMP: *)
+  (*   forall (P: MsgT -> Prop) mind mp, *)
+  (*     ForallMP P mp -> *)
+  (*     ForallMP P (deqMP mind mp). *)
+  (* Proof. *)
+  (*   induction mp; simpl; intros; auto. *)
+  (*   inv H0. *)
+  (*   find_if_inside; auto. *)
+  (*   constructor; auto. *)
+  (*   apply IHmp; auto. *)
+  (* Qed. *)
+
+  (* Lemma ForallMP_removeMP: *)
+  (*   forall (P: MsgT -> Prop) msg mp, *)
+  (*     ForallMP P mp -> *)
+  (*     ForallMP P (removeMP msg mp). *)
+  (* Proof. *)
+  (*   induction mp; simpl; intros; auto. *)
+  (*   inv H0. *)
+  (*   cbn; destruct (isAddrOf _ _ _ _); auto. *)
+  (*   constructor; auto. *)
+  (*   apply ForallMP_deqMP; auto. *)
+  (* Qed. *)
+
+  (* Lemma ForallMP_enqMsgs: *)
+  (*   forall (P: MsgT -> Prop) (nmsgs: list MsgT) mp, *)
+  (*     ForallMP P mp -> *)
+  (*     ForallMP P nmsgs -> *)
+  (*     ForallMP P (enqMsgs nmsgs mp). *)
+  (* Proof. *)
+  (*   intros. *)
+  (*   apply Forall_app; auto. *)
+  (* Qed. *)
+
+  (* Lemma ForallMP_deqMsgs: *)
+  (*   forall (P: MsgT -> Prop) (dmsgs: list MsgT) mp, *)
+  (*     ForallMP P mp -> *)
+  (*     ForallMP P (deqMsgs dmsgs mp). *)
+  (* Proof. *)
+  (*   induction dmsgs; simpl; intros; auto. *)
+  (*   apply IHdmsgs. *)
+  (*   apply ForallMP_removeMP; auto. *)
+  (* Qed. *)
+
+  (* Lemma ForallMP_removeOnce: *)
+  (*   forall (msg_dec: forall m1 m2: MsgT, {m1 = m2} + {m1 <> m2}) *)
+  (*          (P: MsgT -> Prop) tmsg mp, *)
+  (*     ForallMP P mp -> *)
+  (*     ForallMP P (removeOnce msg_dec tmsg mp). *)
+  (* Proof. *)
+  (*   induction mp; simpl; intros; auto. *)
+  (*   inv H0. *)
+  (*   find_if_inside; auto. *)
+  (*   constructor; auto. *)
+  (*   apply IHmp; auto. *)
+  (* Qed. *)
   
-  Lemma deqMP_SubList:
-    forall from to chn mp,
-      SubList (deqMP from to chn mp) mp.
-  Proof.
-    induction mp; simpl; intros; [apply SubList_nil|].
-    find_if_inside.
-    - right; auto.
-    - apply SubList_cons; [left; reflexivity|].
-      apply SubList_cons_right; auto.
-  Qed.
+  (* Lemma deqMP_SubList: *)
+  (*   forall mind mp, *)
+  (*     SubList (deqMP mind mp) mp. *)
+  (* Proof. *)
+  (*   induction mp; simpl; intros; [apply SubList_nil|]. *)
+  (*   find_if_inside. *)
+  (*   - right; auto. *)
+  (*   - apply SubList_cons; [left; reflexivity|]. *)
+  (*     apply SubList_cons_right; auto. *)
+  (* Qed. *)
 
-  Lemma findMP_MsgAddr:
-    forall from to chn msg mp,
-      hd_error (findMP from to chn mp) = Some msg ->
-      mid_addr (msg_id (getMsg msg)) = buildMsgAddr from to chn.
-  Proof.
-    induction mp; simpl; intros; [discriminate|].
-    unfold isAddrOf in H0.
-    destruct (msgAddr_dec _ _); auto.
-    inv H0; auto.
-  Qed.
+  (* Lemma findMP_MsgAddr: *)
+  (*   forall mind msg mp, *)
+  (*     hd_error (findMP mind mp) = Some msg -> *)
+  (*     mid_addr (msg_id (getMsg msg)) = buildMsgAddr mind. *)
+  (* Proof. *)
+  (*   induction mp; simpl; intros; [discriminate|]. *)
+  (*   unfold isAddrOf in H0. *)
+  (*   destruct (msgAddr_dec _ _); auto. *)
+  (*   inv H0; auto. *)
+  (* Qed. *)
 
-  Lemma firstMP_MsgAddr:
-    forall from to chn mp msg,
-      firstMP from to chn mp = Some msg ->
-      mid_addr (msg_id (getMsg msg)) = buildMsgAddr from to chn.
-  Proof.
-    unfold firstMP; intros.
-    eapply findMP_MsgAddr; eauto.
-  Qed.
+  (* Lemma firstMP_MsgAddr: *)
+  (*   forall mind mp msg, *)
+  (*     firstMP mind mp = Some msg -> *)
+  (*     mid_addr (msg_id (getMsg msg)) = buildMsgAddr mind. *)
+  (* Proof. *)
+  (*   unfold firstMP; intros. *)
+  (*   eapply findMP_MsgAddr; eauto. *)
+  (* Qed. *)
 
-  Lemma removeMP_deqMP:
-    forall msg mid mp,
-      msg_id (getMsg msg) = mid ->
-      removeMP msg mp = deqMP (mid_from mid) (mid_to mid) (mid_chn mid) mp.
-  Proof.
-    intros; subst; reflexivity.
-  Qed.
+  (* Lemma removeMP_deqMP: *)
+  (*   forall msg mid mp, *)
+  (*     msg_id (getMsg msg) = mid -> *)
+  (*     removeMP msg mp = deqMP (mid_from mid) (mid_to mid) (mid_chn mid) mp. *)
+  (* Proof. *)
+  (*   intros; subst; reflexivity. *)
+  (* Qed. *)
 
-  Lemma firstMP_FirstMP:
-    forall from to chn mp msg,
-      firstMP from to chn mp = Some msg ->
-      FirstMP mp msg.
-  Proof.
-    unfold FirstMP; intros.
-    pose proof (firstMP_MsgAddr _ _ _ _ H0).
-    destruct (msg_id (getMsg msg)) as [[ ]]; cbn in *.
-    inv H1; assumption.
-  Qed.
+  (* Lemma firstMP_FirstMP: *)
+  (*   forall mind mp msg, *)
+  (*     firstMP mind mp = Some msg -> *)
+  (*     FirstMP mp msg. *)
+  (* Proof. *)
+  (*   unfold FirstMP; intros. *)
+  (*   pose proof (firstMP_MsgAddr _ _ _ _ H0). *)
+  (*   destruct (msg_id (getMsg msg)) as [[ ]]; cbn in *. *)
+  (*   inv H1; assumption. *)
+  (* Qed. *)
 
-  Lemma findMP_nil:
-    forall mp,
-      (forall from to chn, findMP from to chn mp = nil) ->
-      mp = nil.
-  Proof.
-    intros.
-    destruct mp as [|msg ?]; auto.
-    exfalso.
-    specialize (H0 (mid_from (msg_id (getMsg msg)))
-                   (mid_to (msg_id (getMsg msg)))
-                   (mid_chn (msg_id (getMsg msg)))).
-    simpl in H0.
-    unfold isAddrOf in H0.
-    destruct (msgAddr_dec _ _); [discriminate|].
-    elim n.
-    destruct (getMsg msg) as [[[from to chn] tid] val]; cbn in *.
-    reflexivity.
-  Qed.
+  (* Lemma findMP_nil: *)
+  (*   forall mp, *)
+  (*     (forall mind, findMP mind mp = nil) -> *)
+  (*     mp = nil. *)
+  (* Proof. *)
+  (*   intros. *)
+  (*   destruct mp as [|msg ?]; auto. *)
+  (*   exfalso. *)
+  (*   specialize (H0 (mid_from (msg_id (getMsg msg))) *)
+  (*                  (mid_to (msg_id (getMsg msg))) *)
+  (*                  (mid_chn (msg_id (getMsg msg)))). *)
+  (*   simpl in H0. *)
+  (*   unfold isAddrOf in H0. *)
+  (*   destruct (msgAddr_dec _ _); [discriminate|]. *)
+  (*   elim n. *)
+  (*   destruct (getMsg msg) as [[[mind] tid] val]; cbn in *. *)
+  (*   reflexivity. *)
+  (* Qed. *)
 
-  Lemma findMP_app:
-    forall from to chn mp1 mp2,
-      findMP from to chn (mp1 ++ mp2) =
-      findMP from to chn mp1 ++ findMP from to chn mp2.
-  Proof.
-    unfold findMP; intros.
-    apply filter_app.
-  Qed.
+  (* Lemma findMP_app: *)
+  (*   forall mind mp1 mp2, *)
+  (*     findMP mind (mp1 ++ mp2) = *)
+  (*     findMP mind mp1 ++ findMP mind mp2. *)
+  (* Proof. *)
+  (*   unfold findMP; intros. *)
+  (*   apply filter_app. *)
+  (* Qed. *)
 
-  Lemma findMP_SubList:
-    forall from to chn mp,
-      SubList (findMP from to chn mp) mp.
-  Proof.
-    unfold SubList, findMP; intros.
-    apply filter_In in H0; dest; auto.
-  Qed.
+  (* Lemma findMP_SubList: *)
+  (*   forall mind mp, *)
+  (*     SubList (findMP mind mp) mp. *)
+  (* Proof. *)
+  (*   unfold SubList, findMP; intros. *)
+  (*   apply filter_In in H0; dest; auto. *)
+  (* Qed. *)
 
-  Corollary findMP_enqMP:
-    forall from to chn mp msg,
-      findMP from to chn (enqMP msg mp) =
-      findMP from to chn mp ++ findMP from to chn [msg].
-  Proof.
-    unfold enqMP; intros.
-    apply findMP_app.
-  Qed.
+  (* Corollary findMP_enqMP: *)
+  (*   forall mind mp msg, *)
+  (*     findMP mind (enqMP msg mp) = *)
+  (*     findMP mind mp ++ findMP mind [msg]. *)
+  (* Proof. *)
+  (*   unfold enqMP; intros. *)
+  (*   apply findMP_app. *)
+  (* Qed. *)
 
-  Lemma FirstMP_enqMP:
-    forall mp msg,
-      FirstMP mp msg ->
-      forall emsg,
-        FirstMP (enqMP emsg mp) msg.
-  Proof.
-    unfold FirstMP, firstMP, enqMP; intros.
-    rewrite findMP_app.
-    apply hd_error_Some_app; auto.
-  Qed.
+  (* Lemma FirstMP_enqMP: *)
+  (*   forall mp msg, *)
+  (*     FirstMP mp msg -> *)
+  (*     forall emsg, *)
+  (*       FirstMP (enqMP emsg mp) msg. *)
+  (* Proof. *)
+  (*   unfold FirstMP, firstMP, enqMP; intros. *)
+  (*   rewrite findMP_app. *)
+  (*   apply hd_error_Some_app; auto. *)
+  (* Qed. *)
 
-  Lemma FirstMP_distributeMsgs:
-    forall mp msg,
-      FirstMP mp msg ->
-      forall eins,
-        FirstMP (distributeMsgs eins mp) msg.
-  Proof.
-    unfold FirstMP, firstMP, distributeMsgs; intros.
-    rewrite findMP_app.
-    apply hd_error_Some_app; auto.
-  Qed.
+  (* Lemma FirstMP_enqMsgs: *)
+  (*   forall mp msg, *)
+  (*     FirstMP mp msg -> *)
+  (*     forall eins, *)
+  (*       FirstMP (enqMsgs eins mp) msg. *)
+  (* Proof. *)
+  (*   unfold FirstMP, firstMP, enqMsgs; intros. *)
+  (*   rewrite findMP_app. *)
+  (*   apply hd_error_Some_app; auto. *)
+  (* Qed. *)
 
-  Lemma findMP_deqMP_eq:
-    forall from to chn mp,
-      findMP from to chn (deqMP from to chn mp) =
-      deqMP from to chn (findMP from to chn mp).
-  Proof.
-    induction mp; simpl; intros; [reflexivity|].
-    unfold isAddrOf; destruct (msgAddr_dec _ _).
-    - simpl; unfold isAddrOf.
-      destruct (msgAddr_dec _ _); auto.
-      elim n; assumption.
-    - simpl; unfold isAddrOf.
-      destruct (msgAddr_dec _ _); auto.
-      elim n; assumption.
-  Qed.
+  (* Lemma findMP_deqMP_eq: *)
+  (*   forall mind mp, *)
+  (*     findMP mind (deqMP mind mp) = *)
+  (*     deqMP mind (findMP mind mp). *)
+  (* Proof. *)
+  (*   induction mp; simpl; intros; [reflexivity|]. *)
+  (*   unfold isAddrOf; destruct (msgAddr_dec _ _). *)
+  (*   - simpl; unfold isAddrOf. *)
+  (*     destruct (msgAddr_dec _ _); auto. *)
+  (*     elim n; assumption. *)
+  (*   - simpl; unfold isAddrOf. *)
+  (*     destruct (msgAddr_dec _ _); auto. *)
+  (*     elim n; assumption. *)
+  (* Qed. *)
 
-  Lemma findMP_deqMP_neq:
-    forall from to chn dfrom dto dchn mp,
-      buildMsgAddr from to chn <> buildMsgAddr dfrom dto dchn ->
-      findMP from to chn (deqMP dfrom dto dchn mp) =
-      findMP from to chn mp.
-  Proof.
-    induction mp; intros; [reflexivity|].
-    simpl; unfold isAddrOf.
-    destruct (msgAddr_dec _ _).
-    - destruct (msgAddr_dec _ _); auto.
-      rewrite e0 in e; elim H0; assumption.
-    - simpl; unfold isAddrOf.
-      destruct (msgAddr_dec _ _); auto.
-      rewrite e in n.
-      erewrite IHmp; eauto.
-  Qed.
+  (* Lemma findMP_deqMP_neq: *)
+  (*   forall mind dfrom dto dchn mp, *)
+  (*     buildMsgAddr mind <> buildMsgAddr dfrom dto dchn -> *)
+  (*     findMP mind (deqMP dfrom dto dchn mp) = *)
+  (*     findMP mind mp. *)
+  (* Proof. *)
+  (*   induction mp; intros; [reflexivity|]. *)
+  (*   simpl; unfold isAddrOf. *)
+  (*   destruct (msgAddr_dec _ _). *)
+  (*   - destruct (msgAddr_dec _ _); auto. *)
+  (*     rewrite e0 in e; elim H0; assumption. *)
+  (*   - simpl; unfold isAddrOf. *)
+  (*     destruct (msgAddr_dec _ _); auto. *)
+  (*     rewrite e in n. *)
+  (*     erewrite IHmp; eauto. *)
+  (* Qed. *)
 
-  Lemma firstMP_deqMP_app:
-    forall mp1 from to chn,
-      firstMP from to chn mp1 <> None ->
-      forall mp2,
-        deqMP from to chn (mp1 ++ mp2) =
-        deqMP from to chn mp1 ++ mp2.
-  Proof.
-    induction mp1; simpl; intros; [elim H0; reflexivity|].
-    unfold isAddrOf; destruct (msgAddr_dec _ _); auto.
-    simpl; rewrite IHmp1; [reflexivity|].
-    assert (exists v, firstMP from to chn ([a] ++ mp1) = Some v).
-    { simpl.
-      destruct (firstMP from to chn (a :: mp1)); [|exfalso; auto].
-      eexists; reflexivity.
-    }
-    destruct H1 as [v ?].
-    apply firstMP_app_or in H1; destruct H1.
-    - exfalso.
-      unfold firstMP, findMP, isAddrOf in H1; simpl in H1.
-      destruct (msgAddr_dec _ _); auto.
-      discriminate.
-    - rewrite H1; discriminate.
-  Qed.
+  (* Lemma firstMP_deqMP_app: *)
+  (*   forall mp1 mind, *)
+  (*     firstMP mind mp1 <> None -> *)
+  (*     forall mp2, *)
+  (*       deqMP mind (mp1 ++ mp2) = *)
+  (*       deqMP mind mp1 ++ mp2. *)
+  (* Proof. *)
+  (*   induction mp1; simpl; intros; [elim H0; reflexivity|]. *)
+  (*   unfold isAddrOf; destruct (msgAddr_dec _ _); auto. *)
+  (*   simpl; rewrite IHmp1; [reflexivity|]. *)
+  (*   assert (exists v, firstMP mind ([a] ++ mp1) = Some v). *)
+  (*   { simpl. *)
+  (*     destruct (firstMP mind (a :: mp1)); [|exfalso; auto]. *)
+  (*     eexists; reflexivity. *)
+  (*   } *)
+  (*   destruct H1 as [v ?]. *)
+  (*   apply firstMP_app_or in H1; destruct H1. *)
+  (*   - exfalso. *)
+  (*     unfold firstMP, findMP, isAddrOf in H1; simpl in H1. *)
+  (*     destruct (msgAddr_dec _ _); auto. *)
+  (*     discriminate. *)
+  (*   - rewrite H1; discriminate. *)
+  (* Qed. *)
 
-  Lemma FirstMP_deqMP_enqMP_comm:
-    forall mp from to chn emsg,
-      firstMP from to chn mp <> None ->
-      deqMP from to chn (enqMP emsg mp) =
-      enqMP emsg (deqMP from to chn mp).
-  Proof.
-    unfold enqMP; intros.
-    apply firstMP_deqMP_app; auto.
-  Qed.
+  (* Lemma FirstMP_deqMP_enqMP_comm: *)
+  (*   forall mp mind emsg, *)
+  (*     firstMP mind mp <> None -> *)
+  (*     deqMP mind (enqMP emsg mp) = *)
+  (*     enqMP emsg (deqMP mind mp). *)
+  (* Proof. *)
+  (*   unfold enqMP; intros. *)
+  (*   apply firstMP_deqMP_app; auto. *)
+  (* Qed. *)
 
-  Lemma FirstMP_deqMP_distributeMsgs_comm:
-    forall mp from to chn mins,
-      firstMP from to chn mp <> None ->
-      deqMP from to chn (distributeMsgs mins mp) =
-      distributeMsgs mins (deqMP from to chn mp).
-  Proof.
-    unfold enqMP; intros.
-    apply firstMP_deqMP_app; auto.
-  Qed.
+  (* Lemma FirstMP_deqMP_enqMsgs_comm: *)
+  (*   forall mp mind mins, *)
+  (*     firstMP mind mp <> None -> *)
+  (*     deqMP mind (enqMsgs mins mp) = *)
+  (*     enqMsgs mins (deqMP mind mp). *)
+  (* Proof. *)
+  (*   unfold enqMP; intros. *)
+  (*   apply firstMP_deqMP_app; auto. *)
+  (* Qed. *)
 
-  Lemma FirstMP_removeMP_enqMP_comm:
-    forall mp rmsg,
-      FirstMP mp rmsg ->
-      forall emsg,
-        removeMP rmsg (enqMP emsg mp) =
-        enqMP emsg (removeMP rmsg mp).
-  Proof.
-    unfold removeMP; intros.
-    apply FirstMP_deqMP_enqMP_comm.
-    rewrite H0; discriminate.
-  Qed.
+  (* Lemma FirstMP_removeMP_enqMP_comm: *)
+  (*   forall mp rmsg, *)
+  (*     FirstMP mp rmsg -> *)
+  (*     forall emsg, *)
+  (*       removeMP rmsg (enqMP emsg mp) = *)
+  (*       enqMP emsg (removeMP rmsg mp). *)
+  (* Proof. *)
+  (*   unfold removeMP; intros. *)
+  (*   apply FirstMP_deqMP_enqMP_comm. *)
+  (*   rewrite H0; discriminate. *)
+  (* Qed. *)
 
-  Lemma FirstMP_removeMP_distributeMsgs_comm:
-    forall mp rmsg,
-      FirstMP mp rmsg ->
-      forall mins,
-        removeMP rmsg (distributeMsgs mins mp) =
-        distributeMsgs mins (removeMP rmsg mp).
-  Proof.
-    unfold removeMP; intros.
-    apply FirstMP_deqMP_distributeMsgs_comm.
-    rewrite H0; discriminate.
-  Qed.
+  (* Lemma FirstMP_removeMP_enqMsgs_comm: *)
+  (*   forall mp rmsg, *)
+  (*     FirstMP mp rmsg -> *)
+  (*     forall mins, *)
+  (*       removeMP rmsg (enqMsgs mins mp) = *)
+  (*       enqMsgs mins (removeMP rmsg mp). *)
+  (* Proof. *)
+  (*   unfold removeMP; intros. *)
+  (*   apply FirstMP_deqMP_enqMsgs_comm. *)
+  (*   rewrite H0; discriminate. *)
+  (* Qed. *)
 
-  Lemma firstMP'_firstMP'_removeMP:
-    forall mp from1 to1 chn1 msg1 from2 to2 chn2 msg2,
-      buildMsgAddr from1 to1 chn1 <> buildMsgAddr from2 to2 chn2 ->
-      firstMP' from1 to1 chn1 mp = Some msg1 ->
-      firstMP' from2 to2 chn2 mp = Some msg2 ->
-      firstMP' from2 to2 chn2 (removeMP msg1 mp) = Some msg2.
-  Proof.
-    intros.
-    pose proof H1; rewrite <-firstMP_firstMP' in H3.
-    apply firstMP_MsgAddr in H3.
-    pose proof H2; rewrite <-firstMP_firstMP' in H4.
-    apply firstMP_MsgAddr in H4.
-    induction mp; simpl; intros; [discriminate|].
-    cbn in *.
-    remember (getMsg msg1) as m1.
-    destruct m1 as [[[mfrom1 mto1 mchn1] mtid1] mval1]; cbn in *.
-    remember (getMsg msg2) as m2.
-    destruct m2 as [[[mfrom2 mto2 mchn2] mtid2] mval2]; cbn in *.
-    inv H3; inv H4.
-    unfold isAddrOf in *.
-    destruct (msgAddr_dec _ _).
-    - destruct (msgAddr_dec _ _); auto.
-      exfalso; inv H1; inv H2.
-      rewrite e in e0; auto.
-    - simpl; unfold isAddrOf.
-      destruct (msgAddr_dec _ _); auto.
-      specialize (IHmp H1 H2).
-      erewrite removeMP_deqMP in IHmp by reflexivity.
-      rewrite <-Heqm1 in IHmp.
-      assumption.
-  Qed.
+  (* Lemma firstMP'_firstMP'_removeMP: *)
+  (*   forall mp from1 to1 chn1 msg1 from2 to2 chn2 msg2, *)
+  (*     buildMsgAddr from1 to1 chn1 <> buildMsgAddr from2 to2 chn2 -> *)
+  (*     firstMP' from1 to1 chn1 mp = Some msg1 -> *)
+  (*     firstMP' from2 to2 chn2 mp = Some msg2 -> *)
+  (*     firstMP' from2 to2 chn2 (removeMP msg1 mp) = Some msg2. *)
+  (* Proof. *)
+  (*   intros. *)
+  (*   pose proof H1; rewrite <-firstMP_firstMP' in H3. *)
+  (*   apply firstMP_MsgAddr in H3. *)
+  (*   pose proof H2; rewrite <-firstMP_firstMP' in H4. *)
+  (*   apply firstMP_MsgAddr in H4. *)
+  (*   induction mp; simpl; intros; [discriminate|]. *)
+  (*   cbn in *. *)
+  (*   remember (getMsg msg1) as m1. *)
+  (*   destruct m1 as [[[mfrom1 mto1 mchn1] mtid1] mval1]; cbn in *. *)
+  (*   remember (getMsg msg2) as m2. *)
+  (*   destruct m2 as [[[mfrom2 mto2 mchn2] mtid2] mval2]; cbn in *. *)
+  (*   inv H3; inv H4. *)
+  (*   unfold isAddrOf in *. *)
+  (*   destruct (msgAddr_dec _ _). *)
+  (*   - destruct (msgAddr_dec _ _); auto. *)
+  (*     exfalso; inv H1; inv H2. *)
+  (*     rewrite e in e0; auto. *)
+  (*   - simpl; unfold isAddrOf. *)
+  (*     destruct (msgAddr_dec _ _); auto. *)
+  (*     specialize (IHmp H1 H2). *)
+  (*     erewrite removeMP_deqMP in IHmp by reflexivity. *)
+  (*     rewrite <-Heqm1 in IHmp. *)
+  (*     assumption. *)
+  (* Qed. *)
     
-  Lemma FirstMP_FirstMP_removeMP:
-    forall mp msg1 msg2,
-      mid_addr (msg_id (getMsg msg1)) <> mid_addr (msg_id (getMsg msg2)) ->
-      FirstMP mp msg1 ->
-      FirstMP mp msg2 ->
-      FirstMP (removeMP msg1 mp) msg2.
-  Proof.
-    unfold FirstMP; intros.
-    rewrite firstMP_firstMP' in *.
-    induction mp; simpl; intros; [inv H1|].
-    inv H1.
-    unfold FirstMP in *; intros.
-    eapply firstMP'_firstMP'_removeMP; eauto.
-    destruct (getMsg msg1) as [[[mfrom1 mto1 mchn1] mtid1] mval1]; cbn in *.
-    destruct (getMsg msg2) as [[[mfrom2 mto2 mchn2] mtid2] mval2]; cbn in *.
-    auto.
-  Qed.
+  (* Lemma FirstMP_FirstMP_removeMP: *)
+  (*   forall mp msg1 msg2, *)
+  (*     mid_addr (msg_id (getMsg msg1)) <> mid_addr (msg_id (getMsg msg2)) -> *)
+  (*     FirstMP mp msg1 -> *)
+  (*     FirstMP mp msg2 -> *)
+  (*     FirstMP (removeMP msg1 mp) msg2. *)
+  (* Proof. *)
+  (*   unfold FirstMP; intros. *)
+  (*   rewrite firstMP_firstMP' in *. *)
+  (*   induction mp; simpl; intros; [inv H1|]. *)
+  (*   inv H1. *)
+  (*   unfold FirstMP in *; intros. *)
+  (*   eapply firstMP'_firstMP'_removeMP; eauto. *)
+  (*   destruct (getMsg msg1) as [[[mfrom1 mto1 mchn1] mtid1] mval1]; cbn in *. *)
+  (*   destruct (getMsg msg2) as [[[mfrom2 mto2 mchn2] mtid2] mval2]; cbn in *. *)
+  (*   auto. *)
+  (* Qed. *)
 
-  Corollary FirstMP_Forall_FirstMP_removeMP:
-    forall mp msg1 msgs2,
-      Forall (fun msg2 => mid_addr (msg_id (getMsg msg1)) <>
-                          mid_addr (msg_id (getMsg msg2))) msgs2 ->
-      FirstMP mp msg1 ->
-      Forall (FirstMP mp) msgs2 ->
-      Forall (FirstMP (removeMP msg1 mp)) msgs2.
-  Proof.
-    induction msgs2; simpl; intros; [constructor|].
-    inv H0; inv H2.
-    constructor; auto.
-    apply FirstMP_FirstMP_removeMP; auto.
-  Qed.
+  (* Corollary FirstMP_Forall_FirstMP_removeMP: *)
+  (*   forall mp msg1 msgs2, *)
+  (*     Forall (fun msg2 => mid_addr (msg_id (getMsg msg1)) <> *)
+  (*                         mid_addr (msg_id (getMsg msg2))) msgs2 -> *)
+  (*     FirstMP mp msg1 -> *)
+  (*     Forall (FirstMP mp) msgs2 -> *)
+  (*     Forall (FirstMP (removeMP msg1 mp)) msgs2. *)
+  (* Proof. *)
+  (*   induction msgs2; simpl; intros; [constructor|]. *)
+  (*   inv H0; inv H2. *)
+  (*   constructor; auto. *)
+  (*   apply FirstMP_FirstMP_removeMP; auto. *)
+  (* Qed. *)
 
-  Lemma FirstMP_removeMsgs_enqMP_comm:
-    forall msgs mp,
-      NoDup (map (fun msg => mid_addr (msg_id (getMsg msg))) msgs) ->
-      Forall (FirstMP mp) msgs ->
-      forall msg,
-        removeMsgs msgs (enqMP msg mp) =
-        enqMP msg (removeMsgs msgs mp).
-  Proof.
-    induction msgs; simpl; intros; [reflexivity|].
-    inv H0; inv H1.
-    rewrite FirstMP_removeMP_enqMP_comm by assumption.
-    rewrite <-IHmsgs; [reflexivity|assumption|].
-    apply FirstMP_Forall_FirstMP_removeMP; auto.
+  (* Lemma FirstMP_deqMsgs_enqMP_comm: *)
+  (*   forall msgs mp, *)
+  (*     NoDup (map (fun msg => mid_addr (msg_id (getMsg msg))) msgs) -> *)
+  (*     Forall (FirstMP mp) msgs -> *)
+  (*     forall msg, *)
+  (*       deqMsgs msgs (enqMP msg mp) = *)
+  (*       enqMP msg (deqMsgs msgs mp). *)
+  (* Proof. *)
+  (*   induction msgs; simpl; intros; [reflexivity|]. *)
+  (*   inv H0; inv H1. *)
+  (*   rewrite FirstMP_removeMP_enqMP_comm by assumption. *)
+  (*   rewrite <-IHmsgs; [reflexivity|assumption|]. *)
+  (*   apply FirstMP_Forall_FirstMP_removeMP; auto. *)
 
-    clear -H4.
-    induction msgs; [constructor|].
-    constructor.
-    - intro Hx; elim H4; left; auto.
-    - eapply IHmsgs.
-      intro Hx; elim H4; right; auto.
-  Qed.
+  (*   clear -H4. *)
+  (*   induction msgs; [constructor|]. *)
+  (*   constructor. *)
+  (*   - intro Hx; elim H4; left; auto. *)
+  (*   - eapply IHmsgs. *)
+  (*     intro Hx; elim H4; right; auto. *)
+  (* Qed. *)
 
-  Lemma FirstMP_removeMsgs_distributeMsgs_comm:
-    forall msgs mp,
-      NoDup (map (fun msg => mid_addr (msg_id (getMsg msg))) msgs) ->
-      Forall (FirstMP mp) msgs ->
-      forall mins,
-        removeMsgs msgs (distributeMsgs mins mp) =
-        distributeMsgs mins (removeMsgs msgs mp).
-  Proof.
-    induction msgs; simpl; intros; [reflexivity|].
-    inv H0; inv H1.
-    rewrite FirstMP_removeMP_distributeMsgs_comm by assumption.
-    rewrite <-IHmsgs; [reflexivity|assumption|].
-    apply FirstMP_Forall_FirstMP_removeMP; auto.
+  (* Lemma FirstMP_deqMsgs_enqMsgs_comm: *)
+  (*   forall msgs mp, *)
+  (*     NoDup (map (fun msg => mid_addr (msg_id (getMsg msg))) msgs) -> *)
+  (*     Forall (FirstMP mp) msgs -> *)
+  (*     forall mins, *)
+  (*       deqMsgs msgs (enqMsgs mins mp) = *)
+  (*       enqMsgs mins (deqMsgs msgs mp). *)
+  (* Proof. *)
+  (*   induction msgs; simpl; intros; [reflexivity|]. *)
+  (*   inv H0; inv H1. *)
+  (*   rewrite FirstMP_removeMP_enqMsgs_comm by assumption. *)
+  (*   rewrite <-IHmsgs; [reflexivity|assumption|]. *)
+  (*   apply FirstMP_Forall_FirstMP_removeMP; auto. *)
 
-    clear -H4.
-    induction msgs; [constructor|].
-    constructor.
-    - intro Hx; elim H4; left; auto.
-    - eapply IHmsgs.
-      intro Hx; elim H4; right; auto.
-  Qed.
+  (*   clear -H4. *)
+  (*   induction msgs; [constructor|]. *)
+  (*   constructor. *)
+  (*   - intro Hx; elim H4; left; auto. *)
+  (*   - eapply IHmsgs. *)
+  (*     intro Hx; elim H4; right; auto. *)
+  (* Qed. *)
 
 End Facts.
+
+Global Opaque ForallMP.
+
 
 Section Map.
   Variables (MsgT1 MsgT2: Type).
@@ -624,284 +701,284 @@ Section Map.
   Variable (mmap: MsgT1 -> MsgT2).
   Hypothesis (Hmmap: forall msg, getMsg (mmap msg) = getMsg msg).
 
-  Lemma mmap_findMP:
-    forall from to chn mp,
-      findMP from to chn (map mmap mp) =
-      map mmap (findMP from to chn mp).
-  Proof.
-    induction mp; simpl; intros; auto.
-    unfold isAddrOf in *.
-    rewrite IHmp.
-    rewrite Hmmap.
-    destruct (msgAddr_dec _ _); auto.
-  Qed.
+  (* Lemma mmap_findMP: *)
+  (*   forall mind mp, *)
+  (*     findMP mind (map mmap mp) = *)
+  (*     map mmap (findMP mind mp). *)
+  (* Proof. *)
+  (*   induction mp; simpl; intros; auto. *)
+  (*   unfold isAddrOf in *. *)
+  (*   rewrite IHmp. *)
+  (*   rewrite Hmmap. *)
+  (*   destruct (msgAddr_dec _ _); auto. *)
+  (* Qed. *)
 
-  Lemma mmap_firstMP:
-    forall from to chn mp,
-      firstMP from to chn (map mmap mp) =
-      lift mmap (firstMP from to chn mp).
-  Proof.
-    unfold firstMP; intros.
-    rewrite mmap_findMP.
-    apply eq_sym, lift_hd_error.
-  Qed.
+  (* Lemma mmap_firstMP: *)
+  (*   forall mind mp, *)
+  (*     firstMP mind (map mmap mp) = *)
+  (*     lift mmap (firstMP mind mp). *)
+  (* Proof. *)
+  (*   unfold firstMP; intros. *)
+  (*   rewrite mmap_findMP. *)
+  (*   apply eq_sym, lift_hd_error. *)
+  (* Qed. *)
 
-  Lemma mmap_FirstMP:
-    forall mp msg,
-      FirstMP mp msg ->
-      FirstMP (map mmap mp) (mmap msg).
-  Proof.
-    unfold FirstMP; intros.
-    rewrite mmap_firstMP.
-    rewrite Hmmap.
-    rewrite H1.
-    reflexivity.
-  Qed.
+  (* Lemma mmap_FirstMP: *)
+  (*   forall mp msg, *)
+  (*     FirstMP mp msg -> *)
+  (*     FirstMP (map mmap mp) (mmap msg). *)
+  (* Proof. *)
+  (*   unfold FirstMP; intros. *)
+  (*   rewrite mmap_firstMP. *)
+  (*   rewrite Hmmap. *)
+  (*   rewrite H1. *)
+  (*   reflexivity. *)
+  (* Qed. *)
 
-  Lemma mmap_deqMP:
-    forall mp from to chn,
-      map mmap (deqMP from to chn mp) =
-      deqMP from to chn (map mmap mp).
-  Proof.
-    induction mp; simpl; intros; auto.
-    unfold isAddrOf in *.
-    rewrite Hmmap.
-    destruct (msgAddr_dec _ _); auto.
-    simpl; rewrite IHmp; auto.
-  Qed.
+  (* Lemma mmap_deqMP: *)
+  (*   forall mp mind, *)
+  (*     map mmap (deqMP mind mp) = *)
+  (*     deqMP mind (map mmap mp). *)
+  (* Proof. *)
+  (*   induction mp; simpl; intros; auto. *)
+  (*   unfold isAddrOf in *. *)
+  (*   rewrite Hmmap. *)
+  (*   destruct (msgAddr_dec _ _); auto. *)
+  (*   simpl; rewrite IHmp; auto. *)
+  (* Qed. *)
   
-  Lemma mmap_removeMP:
-    forall mp msg,
-      map mmap (removeMP msg mp) =
-      removeMP (mmap msg) (map mmap mp).
-  Proof.
-    unfold removeMP; intros.
-    rewrite Hmmap.
-    apply mmap_deqMP.
-  Qed.
+  (* Lemma mmap_removeMP: *)
+  (*   forall mp msg, *)
+  (*     map mmap (removeMP msg mp) = *)
+  (*     removeMP (mmap msg) (map mmap mp). *)
+  (* Proof. *)
+  (*   unfold removeMP; intros. *)
+  (*   rewrite Hmmap. *)
+  (*   apply mmap_deqMP. *)
+  (* Qed. *)
 
-  Lemma mmap_removeMsgs:
-    forall msgs mp,
-      map mmap (removeMsgs msgs mp) =
-      removeMsgs (map mmap msgs) (map mmap mp).
-  Proof.
-    induction msgs; simpl; intros; auto.
-    rewrite IHmsgs.
-    rewrite mmap_removeMP.
-    reflexivity.
-  Qed.
+  (* Lemma mmap_deqMsgs: *)
+  (*   forall msgs mp, *)
+  (*     map mmap (deqMsgs msgs mp) = *)
+  (*     deqMsgs (map mmap msgs) (map mmap mp). *)
+  (* Proof. *)
+  (*   induction msgs; simpl; intros; auto. *)
+  (*   rewrite IHmsgs. *)
+  (*   rewrite mmap_removeMP. *)
+  (*   reflexivity. *)
+  (* Qed. *)
 
-  Lemma mmap_distributeMsgs:
-    forall mp msgs,
-      map mmap (distributeMsgs msgs mp) =
-      distributeMsgs (map mmap msgs) (map mmap mp).
-  Proof.
-    unfold distributeMsgs; intros.
-    apply map_app.
-  Qed.
+  (* Lemma mmap_enqMsgs: *)
+  (*   forall mp msgs, *)
+  (*     map mmap (enqMsgs msgs mp) = *)
+  (*     enqMsgs (map mmap msgs) (map mmap mp). *)
+  (* Proof. *)
+  (*   unfold enqMsgs; intros. *)
+  (*   apply map_app. *)
+  (* Qed. *)
   
 End Map.
 
-Section EquivMP.
-  Variable (MsgT: Type).
-  Context `{HasMsg MsgT}.
+(* Section EquivMP. *)
+(*   Variable (MsgT: Type). *)
+(*   Context `{HasMsg MsgT}. *)
   
-  (* Every [Queue] is equal. *)
-  Definition EquivMP (m1 m2: MessagePool MsgT) :=
-    forall from to chn,
-      findMP from to chn m1 = findMP from to chn m2.
+(*   (* Every [Queue] is equal. *) *)
+(*   Definition EquivMP (m1 m2: MessagePool MsgT) := *)
+(*     forall mind, *)
+(*       findMP mind m1 = findMP mind m2. *)
 
-End EquivMP.
+(* End EquivMP. *)
 
-Section EquivMPFacts.
-  Variable (MsgT: Type).
-  Context `{HasMsg MsgT}.
+(* Section EquivMPFacts. *)
+(*   Variable (MsgT: Type). *)
+(*   Context `{HasMsg MsgT}. *)
 
-  Lemma EquivMP_refl:
-    forall mp, EquivMP mp mp.
-  Proof.
-    unfold EquivMP; intros; reflexivity.
-  Qed.
+(*   Lemma EquivMP_refl: *)
+(*     forall mp, EquivMP mp mp. *)
+(*   Proof. *)
+(*     unfold EquivMP; intros; reflexivity. *)
+(*   Qed. *)
 
-  Lemma EquivMP_sym:
-    forall mp1 mp2, EquivMP mp1 mp2 -> EquivMP mp2 mp1.
-  Proof.
-    unfold EquivMP; intros; auto.
-  Qed.
+(*   Lemma EquivMP_sym: *)
+(*     forall mp1 mp2, EquivMP mp1 mp2 -> EquivMP mp2 mp1. *)
+(*   Proof. *)
+(*     unfold EquivMP; intros; auto. *)
+(*   Qed. *)
 
-  Lemma EquivMP_trans:
-    forall mp1 mp2 mp3,
-      EquivMP mp1 mp2 ->
-      EquivMP mp2 mp3 ->
-      EquivMP mp1 mp3.
-  Proof.
-    unfold EquivMP; intros.
-    rewrite H0; auto.
-  Qed.
+(*   Lemma EquivMP_trans: *)
+(*     forall mp1 mp2 mp3, *)
+(*       EquivMP mp1 mp2 -> *)
+(*       EquivMP mp2 mp3 -> *)
+(*       EquivMP mp1 mp3. *)
+(*   Proof. *)
+(*     unfold EquivMP; intros. *)
+(*     rewrite H0; auto. *)
+(*   Qed. *)
 
-  Lemma EquivMP_enqMP:
-    forall mp1 mp2,
-      EquivMP mp1 mp2 ->
-      forall msg,
-        EquivMP (enqMP msg mp1) (enqMP msg mp2).
-  Proof.
-    unfold EquivMP; intros.
-    do 2 rewrite findMP_enqMP.
-    rewrite H0; reflexivity.
-  Qed.
+(*   Lemma EquivMP_enqMP: *)
+(*     forall mp1 mp2, *)
+(*       EquivMP mp1 mp2 -> *)
+(*       forall msg, *)
+(*         EquivMP (enqMP msg mp1) (enqMP msg mp2). *)
+(*   Proof. *)
+(*     unfold EquivMP; intros. *)
+(*     do 2 rewrite findMP_enqMP. *)
+(*     rewrite H0; reflexivity. *)
+(*   Qed. *)
 
-  Lemma EquivMP_FirstMP:
-    forall mp1 mp2,
-      EquivMP mp1 mp2 ->
-      forall msg,
-        FirstMP mp1 msg ->
-        FirstMP mp2 msg.
-  Proof.
-    unfold EquivMP, FirstMP, firstMP; intros.
-    rewrite <-H0; assumption.
-  Qed.
+(*   Lemma EquivMP_FirstMP: *)
+(*     forall mp1 mp2, *)
+(*       EquivMP mp1 mp2 -> *)
+(*       forall msg, *)
+(*         FirstMP mp1 msg -> *)
+(*         FirstMP mp2 msg. *)
+(*   Proof. *)
+(*     unfold EquivMP, FirstMP, firstMP; intros. *)
+(*     rewrite <-H0; assumption. *)
+(*   Qed. *)
 
-  Corollary EquivMP_Forall_FirstMP:
-    forall mp1 mp2,
-      EquivMP mp1 mp2 ->
-      forall msgs,
-        Forall (FirstMP mp1) msgs ->
-        Forall (FirstMP mp2) msgs.
-  Proof.
-    intros.
-    eapply Forall_impl; [|eassumption].
-    intros.
-    eapply EquivMP_FirstMP; eauto.
-  Qed.
+(*   Corollary EquivMP_Forall_FirstMP: *)
+(*     forall mp1 mp2, *)
+(*       EquivMP mp1 mp2 -> *)
+(*       forall msgs, *)
+(*         Forall (FirstMP mp1) msgs -> *)
+(*         Forall (FirstMP mp2) msgs. *)
+(*   Proof. *)
+(*     intros. *)
+(*     eapply Forall_impl; [|eassumption]. *)
+(*     intros. *)
+(*     eapply EquivMP_FirstMP; eauto. *)
+(*   Qed. *)
 
-  Lemma EquivMP_distributeMsgs:
-    forall mp1 mp2,
-      EquivMP mp1 mp2 ->
-      forall msgs,
-        EquivMP (distributeMsgs msgs mp1) (distributeMsgs msgs mp2).
-  Proof.
-    unfold EquivMP, distributeMsgs; intros.
-    do 2 rewrite findMP_app.
-    rewrite H0; reflexivity.
-  Qed.
+(*   Lemma EquivMP_enqMsgs: *)
+(*     forall mp1 mp2, *)
+(*       EquivMP mp1 mp2 -> *)
+(*       forall msgs, *)
+(*         EquivMP (enqMsgs msgs mp1) (enqMsgs msgs mp2). *)
+(*   Proof. *)
+(*     unfold EquivMP, enqMsgs; intros. *)
+(*     do 2 rewrite findMP_app. *)
+(*     rewrite H0; reflexivity. *)
+(*   Qed. *)
 
-  Lemma EquivMP_deqMP:
-    forall mp1 mp2,
-      EquivMP mp1 mp2 ->
-      forall from to chn,
-        EquivMP (deqMP from to chn mp1) (deqMP from to chn mp2).
-  Proof.
-    unfold EquivMP; intros.
-    destruct (msgAddr_dec (buildMsgAddr from0 to0 chn0) (buildMsgAddr from to chn)).
-    - inv e.
-      do 2 rewrite findMP_deqMP_eq.
-      rewrite H0; reflexivity.
-    - do 2 rewrite findMP_deqMP_neq by assumption.
-      auto.
-  Qed.
+(*   Lemma EquivMP_deqMP: *)
+(*     forall mp1 mp2, *)
+(*       EquivMP mp1 mp2 -> *)
+(*       forall mind, *)
+(*         EquivMP (deqMP mind mp1) (deqMP mind mp2). *)
+(*   Proof. *)
+(*     unfold EquivMP; intros. *)
+(*     destruct (msgAddr_dec (buildMsgAddr from0 to0 chn0) (buildMsgAddr mind)). *)
+(*     - inv e. *)
+(*       do 2 rewrite findMP_deqMP_eq. *)
+(*       rewrite H0; reflexivity. *)
+(*     - do 2 rewrite findMP_deqMP_neq by assumption. *)
+(*       auto. *)
+(*   Qed. *)
 
-  Lemma EquivMP_removeMP:
-    forall mp1 mp2,
-      EquivMP mp1 mp2 ->
-      forall msg,
-        EquivMP (removeMP msg mp1) (removeMP msg mp2).
-  Proof.
-    intros; apply EquivMP_deqMP; auto.
-  Qed.
+(*   Lemma EquivMP_removeMP: *)
+(*     forall mp1 mp2, *)
+(*       EquivMP mp1 mp2 -> *)
+(*       forall msg, *)
+(*         EquivMP (removeMP msg mp1) (removeMP msg mp2). *)
+(*   Proof. *)
+(*     intros; apply EquivMP_deqMP; auto. *)
+(*   Qed. *)
 
-  Lemma EquivMP_removeMsgs:
-    forall msgs mp1 mp2,
-      EquivMP mp1 mp2 ->
-      EquivMP (removeMsgs msgs mp1) (removeMsgs msgs mp2).
-  Proof.
-    induction msgs; intros; auto.
-    simpl.
-    apply IHmsgs.
-    apply EquivMP_removeMP.
-    auto.
-  Qed.
+(*   Lemma EquivMP_deqMsgs: *)
+(*     forall msgs mp1 mp2, *)
+(*       EquivMP mp1 mp2 -> *)
+(*       EquivMP (deqMsgs msgs mp1) (deqMsgs msgs mp2). *)
+(*   Proof. *)
+(*     induction msgs; intros; auto. *)
+(*     simpl. *)
+(*     apply IHmsgs. *)
+(*     apply EquivMP_removeMP. *)
+(*     auto. *)
+(*   Qed. *)
 
-  Lemma EquivMP_app:
-    forall mp1 mp2,
-      EquivMP mp1 mp2 ->
-      forall mp3 mp4,
-        EquivMP mp3 mp4 ->
-        EquivMP (mp1 ++ mp3) (mp2 ++ mp4).
-  Proof.
-    unfold EquivMP; intros.
-    do 2 rewrite findMP_app.
-    rewrite H0, H1; reflexivity.
-  Qed.
+(*   Lemma EquivMP_app: *)
+(*     forall mp1 mp2, *)
+(*       EquivMP mp1 mp2 -> *)
+(*       forall mp3 mp4, *)
+(*         EquivMP mp3 mp4 -> *)
+(*         EquivMP (mp1 ++ mp3) (mp2 ++ mp4). *)
+(*   Proof. *)
+(*     unfold EquivMP; intros. *)
+(*     do 2 rewrite findMP_app. *)
+(*     rewrite H0, H1; reflexivity. *)
+(*   Qed. *)
 
-  Lemma MsgAddr_NoDup_not_In_findMP:
-    forall mp,
-      NoDup (map (fun msg => mid_addr (msg_id (getMsg msg))) mp) ->
-      forall from to chn,
-        ~ In (buildMsgAddr from to chn)
-          (map (fun msg => mid_addr (msg_id (getMsg msg))) mp) ->
-        findMP from to chn mp = nil.
-  Proof.
-    induction mp; simpl; intros; [reflexivity|].
-    inv H0; specialize (IHmp H5); clear H5.
-    unfold isAddrOf; destruct (msgAddr_dec _ _); auto.
-    exfalso; eauto.
-  Qed.
+(*   Lemma MsgAddr_NoDup_not_In_findMP: *)
+(*     forall mp, *)
+(*       NoDup (map (fun msg => mid_addr (msg_id (getMsg msg))) mp) -> *)
+(*       forall mind, *)
+(*         ~ In (buildMsgAddr mind) *)
+(*           (map (fun msg => mid_addr (msg_id (getMsg msg))) mp) -> *)
+(*         findMP mind mp = nil. *)
+(*   Proof. *)
+(*     induction mp; simpl; intros; [reflexivity|]. *)
+(*     inv H0; specialize (IHmp H5); clear H5. *)
+(*     unfold isAddrOf; destruct (msgAddr_dec _ _); auto. *)
+(*     exfalso; eauto. *)
+(*   Qed. *)
   
-  Lemma MsgAddr_NoDup_In_findMP:
-    forall mp,
-      NoDup (map (fun msg => mid_addr (msg_id (getMsg msg))) mp) ->
-      forall from to chn,
-        In (buildMsgAddr from to chn) (map (fun msg => mid_addr (msg_id (getMsg msg))) mp) ->
-        exists msg,
-          findMP from to chn mp = [msg] /\
-          mid_addr (msg_id (getMsg msg)) = buildMsgAddr from to chn.
-  Proof.
-    induction mp; simpl; intros; [elim H1|].
-    inv H0; specialize (IHmp H5).
-    unfold isAddrOf; destruct (msgAddr_dec _ _).
-    - exists a; split; auto.
-      rewrite MsgAddr_NoDup_not_In_findMP; auto.
-      rewrite <-e; assumption.
-    - destruct H1; eauto.
-      elim n; assumption.
-  Qed.
+(*   Lemma MsgAddr_NoDup_In_findMP: *)
+(*     forall mp, *)
+(*       NoDup (map (fun msg => mid_addr (msg_id (getMsg msg))) mp) -> *)
+(*       forall mind, *)
+(*         In (buildMsgAddr mind) (map (fun msg => mid_addr (msg_id (getMsg msg))) mp) -> *)
+(*         exists msg, *)
+(*           findMP mind mp = [msg] /\ *)
+(*           mid_addr (msg_id (getMsg msg)) = buildMsgAddr mind. *)
+(*   Proof. *)
+(*     induction mp; simpl; intros; [elim H1|]. *)
+(*     inv H0; specialize (IHmp H5). *)
+(*     unfold isAddrOf; destruct (msgAddr_dec _ _). *)
+(*     - exists a; split; auto. *)
+(*       rewrite MsgAddr_NoDup_not_In_findMP; auto. *)
+(*       rewrite <-e; assumption. *)
+(*     - destruct H1; eauto. *)
+(*       elim n; assumption. *)
+(*   Qed. *)
 
-  Lemma EquivMP_MsgAddr_NoDup_EquivList:
-    forall mp1 mp2,
-      NoDup (map (fun msg => mid_addr (msg_id (getMsg msg))) mp1) ->
-      NoDup (map (fun msg => mid_addr (msg_id (getMsg msg))) mp2) ->
-      EquivList mp1 mp2 ->
-      EquivMP mp1 mp2.
-  Proof.
-    unfold EquivMP; intros.
+(*   Lemma EquivMP_MsgAddr_NoDup_EquivList: *)
+(*     forall mp1 mp2, *)
+(*       NoDup (map (fun msg => mid_addr (msg_id (getMsg msg))) mp1) -> *)
+(*       NoDup (map (fun msg => mid_addr (msg_id (getMsg msg))) mp2) -> *)
+(*       EquivList mp1 mp2 -> *)
+(*       EquivMP mp1 mp2. *)
+(*   Proof. *)
+(*     unfold EquivMP; intros. *)
 
-    assert (EquivList (map (fun msg => mid_addr (msg_id (getMsg msg))) mp1)
-                      (map (fun msg => mid_addr (msg_id (getMsg msg))) mp2)).
-    { destruct H2; split; apply SubList_map; auto. }
+(*     assert (EquivList (map (fun msg => mid_addr (msg_id (getMsg msg))) mp1) *)
+(*                       (map (fun msg => mid_addr (msg_id (getMsg msg))) mp2)). *)
+(*     { destruct H2; split; apply SubList_map; auto. } *)
     
-    destruct (in_dec msgAddr_dec (buildMsgAddr from to chn)
-                     (map (fun msg : MsgT => mid_addr (msg_id (getMsg msg))) mp1));
-      destruct (in_dec msgAddr_dec (buildMsgAddr from to chn)
-                       (map (fun msg : MsgT => mid_addr (msg_id (getMsg msg))) mp2)).
-    - apply MsgAddr_NoDup_In_findMP in i; [|assumption]; destruct i as [msg1].
-      apply MsgAddr_NoDup_In_findMP in i0; [|assumption]; destruct i0 as [msg2].
-      dest; rewrite H4, H5.
+(*     destruct (in_dec msgAddr_dec (buildMsgAddr mind) *)
+(*                      (map (fun msg : MsgT => mid_addr (msg_id (getMsg msg))) mp1)); *)
+(*       destruct (in_dec msgAddr_dec (buildMsgAddr mind) *)
+(*                        (map (fun msg : MsgT => mid_addr (msg_id (getMsg msg))) mp2)). *)
+(*     - apply MsgAddr_NoDup_In_findMP in i; [|assumption]; destruct i as [msg1]. *)
+(*       apply MsgAddr_NoDup_In_findMP in i0; [|assumption]; destruct i0 as [msg2]. *)
+(*       dest; rewrite H4, H5. *)
       
-      pose proof (findMP_SubList from to chn mp1); rewrite H4 in H8.
-      specialize (H8 _ (or_introl eq_refl)).
-      pose proof (findMP_SubList from to chn mp2); rewrite H5 in H9.
-      specialize (H9 _ (or_introl eq_refl)).
-      assert (msg1 = msg2).
-      { eapply NoDup_map_In; eauto.
-        { apply H2; auto. }
-        { simpl; rewrite H6, H7; reflexivity. }
-      }
-      subst; reflexivity.
-    - elim n; apply H3; assumption.
-    - elim n; apply H3; assumption.
-    - do 2 (rewrite MsgAddr_NoDup_not_In_findMP by assumption).
-      reflexivity.
-  Qed.
+(*       pose proof (findMP_SubList mind mp1); rewrite H4 in H8. *)
+(*       specialize (H8 _ (or_introl eq_refl)). *)
+(*       pose proof (findMP_SubList mind mp2); rewrite H5 in H9. *)
+(*       specialize (H9 _ (or_introl eq_refl)). *)
+(*       assert (msg1 = msg2). *)
+(*       { eapply NoDup_map_In; eauto. *)
+(*         { apply H2; auto. } *)
+(*         { simpl; rewrite H6, H7; reflexivity. } *)
+(*       } *)
+(*       subst; reflexivity. *)
+(*     - elim n; apply H3; assumption. *)
+(*     - elim n; apply H3; assumption. *)
+(*     - do 2 (rewrite MsgAddr_NoDup_not_In_findMP by assumption). *)
+(*       reflexivity. *)
+(*   Qed. *)
 
-End EquivMPFacts.
+(* End EquivMPFacts. *)
 
