src/Invariant.v
@@ -87,16 +87,22 @@ Infix "->i" := invImp (at level 99).
 (*! Some generic invariants *)
 
 Definition MsgsInInv (inv: TState -> Prop) :=
-  forall oss orqs msgs ts eins,
-    inv {| tst_oss := oss; tst_orqs := orqs; tst_msgs := msgs; tst_tid := ts |} ->
+  forall oss orqs msgs trss trss' ts eins,
     inv {| tst_oss := oss; tst_orqs := orqs;
-           tst_msgs := distributeMsgs (toTMsgsU eins) msgs; tst_tid := ts |}.
+           tst_msgs := msgs; tst_trss := trss; tst_tid := ts |} ->
+    inv {| tst_oss := oss; tst_orqs := orqs;
+           tst_msgs := enqMsgs (imap toTMsgU eins) msgs;
+           tst_trss := trss';
+           tst_tid := ts |}.
 
 Definition MsgsOutInv (inv: TState -> Prop) :=
-  forall oss orqs msgs ts eouts,
-    inv {| tst_oss := oss; tst_orqs := orqs; tst_msgs := msgs; tst_tid := ts |} ->
+  forall oss orqs msgs trss trss' ts eouts,
     inv {| tst_oss := oss; tst_orqs := orqs;
-           tst_msgs := removeMsgs eouts msgs; tst_tid := ts |}.
+           tst_msgs := msgs; tst_trss := trss; tst_tid := ts |} ->
+    inv {| tst_oss := oss; tst_orqs := orqs;
+           tst_msgs := deqMsgs eouts msgs;
+           tst_trss := trss';
+           tst_tid := ts |}.
 
 Definition MsgsInv := MsgsInInv /\i MsgsOutInv.
 
@@ -145,7 +151,7 @@ Section Facts.
   Proof.
     intros; hnf; intros.
     destruct H.
-    inv H2; auto.
+    inv H2; eauto.
     exfalso.
     rewrite H0 in H11.
     elim H11.
@@ -158,12 +164,6 @@ Definition WfDomOStates (dom: list IdxT) (oss: OStates) :=
 
 Definition WfDomTState (dom: list IdxT) (tst: TState) :=
   WfDomOStates dom (tst_oss tst).
-
-Definition TInfoExists (sys: System) (tst: TState) :=
-  ForallMP (fun tmsg =>
-              if fromInternal sys tmsg
-              then tmsg_info tmsg <> None
-              else tmsg_info tmsg = None) (tst_msgs tst).
 
 Definition TidLeMP (tmsgs: MessagePool TMsg) (tid: TrsId) :=
   ForallMP (fun tmsg =>
@@ -188,26 +188,15 @@ Definition TidLt (tid: TrsId) (tst: TState) :=
 Definition ValidTidState (tst: TState) :=
   TidLe (tst_tid tst) tst.
 
-Definition NoExtOutsMP (sys: System) (tmsgs: MessagePool TMsg) :=
-  Forall (fun tmsg => toExternal sys tmsg = false) tmsgs.
-
-Definition NoExtOuts (sys: System) (tst: TState) :=
-  NoExtOutsMP sys (tst_msgs tst).
-
 Lemma ValidTidState_MsgsInv:
   MsgsInv ValidTidState.
 Proof.
-  hnf; intros.
-  split.
-  - hnf; intros; hnf in H; intros.
-    cbn in *.
-    apply Forall_app; auto.
-    clear; induction eins; [constructor|].
-    simpl; constructor; simpl; auto.
-  - hnf; intros; hnf in H; intros.
-    cbn in *.
-    hnf; cbn.
-    apply ForallMP_removeMsgs; auto.
+  split; hnf; intros; hnf in *; cbn in *.
+  - apply ForallMP_enqMsgs; auto.
+    clear; induction eins; simpl; auto.
+    constructor; auto.
+    cbn; auto.
+  - apply ForallMP_deqMsgs; auto.
 Qed.
 
 Lemma step_t_ValidTidState:
@@ -217,35 +206,33 @@ Lemma step_t_ValidTidState:
       step_t sys st1 lbl st2 ->
       ValidTidState st2.
 Proof.
-  unfold ValidTidState; intros; inv H0; auto.
-  - simpl; simpl in H.
-    apply ForallMP_distributeMsgs; auto.
+  unfold ValidTidState; intros.
+  inv H0; auto.
+  - hnf; hnf in H; simpl in *.
+    apply ForallMP_enqMsgs; auto.
     clear; induction eins; [constructor|].
     constructor; simpl; auto.
-  - simpl; simpl in H.
-    apply ForallMP_removeMsgs; auto.
-  - simpl; simpl in H.
-    apply ForallMP_distributeMsgs.
-    + apply ForallMP_removeMsgs.
-      clear -H Hts.
-      induction msgs; simpl; [constructor|].
-      inv H; constructor.
-      * destruct (tmsg_info a); auto.
-        destruct (getTMsgsTInfo ins); omega.
-      * apply IHmsgs; auto.
-    + apply Forall_impl with (Q:= fun msg => InMP msg msgs) in H5;
+  - hnf; hnf in H; simpl in *.
+    apply ForallMP_deqMsgs; auto.
+  - hnf; hnf in H; simpl in *.
+    apply ForallMP_enqMsgs.
+    + apply ForallMP_deqMsgs.
+      eapply ForallMP_impl; eauto.
+      clear -Hts; simpl; intros.
+      destruct (tmsg_info m); auto.
+      destruct (getTMsgsTInfo _); auto.
+      omega.
+    + apply Forall_impl with (Q:= fun idt => InMP (fst idt) (snd idt) msgs) in H5;
         [|intros; eapply FirstMP_InMP; eauto].
-      apply ForallMP_InMP_SubList in H5.
-      eapply ForallMP_SubList in H5; eauto.
+      eapply ForallMP_Forall_InMP in H5; eauto.
 
       clear -Hts H5.
       induction outs; [constructor|].
       constructor; auto.
-
-      simpl; remember (getTMsgsTInfo ins) as ti; destruct ti; auto.
+      simpl; remember (getTMsgsTInfo (valsOf ins)) as ti; destruct ti; auto.
       apply eq_sym, getTMsgsTInfo_Some in Heqti.
       destruct Heqti as [tmsg [? ?]].
-      eapply ForallMP_forall in H5; eauto.
+      eapply Forall_forall in H5; eauto.
       rewrite H0 in H5; auto.
 Qed.
 
@@ -267,9 +254,9 @@ Lemma TidLe_TidLt:
     TidLt nts tst.
 Proof.
   unfold TidLe, TidLt, TidLeMP, TidLtMP; intros.
-  eapply Forall_impl; eauto.
+  eapply ForallMP_impl; eauto.
   simpl; intros.
-  destruct (tmsg_info a); auto.
+  destruct (tmsg_info m); auto.
   omega.
 Qed.
 
@@ -278,7 +265,7 @@ Lemma step_t_TidLt:
     ValidTidState st1 ->
     mins <> nil ->
     step_t sys st1 (RlblInt orule mins mouts) st2 ->
-    Forall (fun tmsg => tmsg_info tmsg = None) mins ->
+    Forall (fun tmsg => tmsg_info tmsg = None) (valsOf mins) ->
     TidLt (tst_tid st2) st1.
 Proof.
   intros; inv H1; [elim H0; reflexivity|].
@@ -291,11 +278,11 @@ Corollary step_t_tid_next_TidLt:
     ValidTidState st1 ->
     step_t sys st1 (RlblInt orule ins outs) st2 ->
     ins <> nil -> outs <> nil ->
-    Forall (fun tmsg => tmsg_info tmsg = None) ins ->
+    Forall (fun tmsg => tmsg_info tmsg = None) (valsOf ins) ->
     Forall (fun tmsg => match tmsg_info tmsg with
                         | Some ti => tinfo_tid ti = ts
                         | None => True
-                        end) outs ->
+                        end) (valsOf outs) ->
     TidLt ts st1.
 Proof.
   intros.
@@ -304,66 +291,26 @@ Proof.
   - eauto using step_t_tid_next.
 Qed.
 
-Lemma validMsgOuts_from_internal:
-  forall {MsgT} `{HasMsg MsgT} sys idx,
-    isInternal sys idx = true ->
-    forall mouts: list MsgT,
-      ValidMsgsOut idx mouts ->
-      ForallMP (fun msg => fromInternal sys msg = true) mouts.
-Proof.
-  induction mouts; simpl; intros; [constructor|].
-  destruct H1; inv H1; inv H2; inv H5; dest.
-  constructor.
-  - simpl in H0; unfold_idx.
-    rewrite H0; reflexivity.
-  - apply IHmouts; split; auto.
-Qed.
-
-Lemma step_t_tinfo:
-  forall sys st1,
-    TInfoExists sys st1 ->
-    forall lbl st2,
-      step_t sys st1 lbl st2 ->
-      TInfoExists sys st2.
-Proof.
-  unfold TInfoExists; intros; inv H0; auto.
-  - simpl; simpl in H.
-    apply ForallMP_distributeMsgs; auto.
-    destruct H2.
-    clear -H0; induction eins; [constructor|].
-    inv H0; dest.
-    specialize (IHeins H3).
-    simpl; constructor; auto.
-    unfold_idx; simpl.
-    destruct (ma_from _ ?<n _); congruence.
-  - simpl; simpl in H.
-    apply ForallMP_removeMsgs; auto.
-  - simpl; simpl in H.
-    apply ForallMP_distributeMsgs.
-    + apply ForallMP_removeMsgs; auto.
-    + pose proof (idx_in_sys_internal _ _ H2).
-      eapply validMsgOuts_from_internal in H11; eauto.
-      clear -H11; simpl in H11.
-      induction outs; [constructor|].
-      inv H11.
-      simpl; constructor; cbn.
-      * unfold fromInternal in *; simpl in *.
-        unfold id in H1; rewrite H1.
-        discriminate.
-      * apply IHouts; auto.
-Qed.
-
 Lemma step_t_rules_split:
-  forall inds inits rules1 rules2 st1 lbl st2,
-    step_t {| sys_inds := inds;
-                sys_inits := inits;
-                sys_rules := rules1 ++ rules2 |} st1 lbl st2 ->
-    step_t {| sys_inds := inds;
-                sys_inits := inits;
-                sys_rules := rules1 |} st1 lbl st2 \/
-    step_t {| sys_inds := inds;
-                sys_inits := inits;
-                sys_rules := rules2 |} st1 lbl st2.
+  forall oinds minds merqs merss inits rules1 rules2 st1 lbl st2,
+    step_t {| sys_oinds := oinds;
+              sys_minds := minds;
+              sys_merqs := merqs;
+              sys_merss := merss;
+              sys_inits := inits;
+              sys_rules := rules1 ++ rules2 |} st1 lbl st2 ->
+    step_t {| sys_oinds := oinds;
+              sys_minds := minds;
+              sys_merqs := merqs;
+              sys_merss := merss;
+              sys_inits := inits;
+              sys_rules := rules1 |} st1 lbl st2 \/
+    step_t {| sys_oinds := oinds;
+              sys_minds := minds;
+              sys_merqs := merqs;
+              sys_merss := merss;
+              sys_inits := inits;
+              sys_rules := rules2 |} st1 lbl st2.
 Proof.
   intros.
   inv H.
@@ -376,64 +323,3 @@ Proof.
     + right; econstructor; eauto.
 Qed.
 
-Lemma steps_t_tinfo:
-  forall sys st1,
-    TInfoExists sys st1 ->
-    forall hst st2,
-      steps step_t sys st1 hst st2 ->
-      TInfoExists sys st2.
-Proof.
-  induction 2; simpl; intros; auto.
-  apply step_t_tinfo in H1; auto.
-Qed.
-
-Lemma step_t_no_rules_NoExtOuts:
-  forall sys,
-    sys_rules sys = nil ->
-    forall st1,
-      NoExtOuts sys st1 ->
-      forall lbl st2,
-        step_t sys st1 lbl st2 ->
-        NoExtOuts sys st2.
-Proof.
-  unfold NoExtOuts, NoExtOutsMP; intros.
-  inv H1; simpl in *; auto.
-  - apply ForallMP_distributeMsgs; auto.
-    destruct H3.
-    clear -H1; induction eins; simpl; [constructor|].
-    inv H1; dest.
-    constructor.
-    + unfold toInternal, toExternal in *; simpl in *.
-      unfold id in H0.
-      apply internal_not_external; auto.
-    + apply IHeins; auto.
-  - apply ForallMP_removeMsgs; auto.
-  - exfalso.
-    rewrite H in H9; elim H9.
-Qed.
-
-Lemma steps_t_no_rules_NoExtOuts:
-  forall sys,
-    sys_rules sys = nil ->
-    forall st1,
-      NoExtOuts sys st1 ->
-      forall ll st2,
-        steps step_t sys st1 ll st2 ->
-        NoExtOuts sys st2.
-Proof.
-  induction 3; simpl; intros; auto.
-  eapply step_t_no_rules_NoExtOuts with (st1 := st2); eauto.
-Qed.
-
-Corollary behavior_no_rules_NoExtOuts:
-  forall sys,
-    sys_rules sys = nil ->
-    forall ll st,
-      steps step_t sys (initsOf sys) ll st ->
-      NoExtOuts sys st.
-Proof.
-  intros.
-  eapply steps_t_no_rules_NoExtOuts; eauto.
-  constructor.
-Qed.
-  
