src/SemFacts.v
@@ -7,7 +7,7 @@ Set Implicit Arguments.
 
 Lemma addRules_indices:
   forall rules sys,
-    indicesOf (addRules rules sys) = indicesOf sys.
+    oindsOf (addRules rules sys) = oindsOf sys.
 Proof.
   reflexivity.
 Qed.
@@ -26,26 +26,6 @@ Proof.
   reflexivity.
 Qed.
 
-Corollary addRules_isExternal:
-  forall rules sys,
-    isExternal (addRules rules sys) =
-    isExternal sys.
-Proof.
-  unfold isExternal; intros.
-  rewrite addRules_indices.
-  reflexivity.
-Qed.
-  
-Corollary addRules_isInternal:
-  forall rules sys,
-    isInternal (addRules rules sys) =
-    isInternal sys.
-Proof.
-  unfold isInternal; intros.
-  rewrite addRules_indices.
-  reflexivity.
-Qed.
-
 Corollary addRules_behaviorOf:
   forall sys rules hst,
     behaviorOf (addRules rules sys) hst = behaviorOf sys hst.
@@ -54,29 +34,11 @@ Proof.
   simpl; rewrite IHhst; reflexivity.
 Qed.
 
-Lemma buildRawSys_indicesOf:
+Lemma buildRawSys_oindsOf:
   forall {SysT} `{IsSystem SysT} `{HasInit SysT OStates} (sys: SysT),
-    indicesOf sys = indicesOf (buildRawSys sys).
+    oindsOf sys = oindsOf (buildRawSys sys).
 Proof.
-  intros; unfold indicesOf, buildRawSys; simpl.
-  reflexivity.
-Qed.
-
-Corollary buildRawSys_isExternal:
-  forall {SysT} `{IsSystem SysT} `{HasInit SysT OStates} (sys: SysT),
-    isExternal (buildRawSys sys) = isExternal sys.
-Proof.
-  unfold isExternal; intros.
-  rewrite <-buildRawSys_indicesOf.
-  reflexivity.
-Qed.
-
-Corollary buildRawSys_isInternal:
-  forall {SysT} `{IsSystem SysT} `{HasInit SysT OStates} (sys: SysT),
-    isInternal (buildRawSys sys) = isInternal sys.
-Proof.
-  unfold isInternal; intros.
-  rewrite <-buildRawSys_indicesOf.
+  intros; unfold oindsOf, buildRawSys; simpl.
   reflexivity.
 Qed.
 
@@ -91,7 +53,7 @@ Qed.
 
 Lemma addRulesSys_buildRawSys:
   forall rules sys,
-    rulesOf (addRules rules (buildRawSys sys)) = rules.
+    sys_rules (addRules rules (buildRawSys sys)) = rules.
 Proof.
   reflexivity.
 Qed.
@@ -129,416 +91,41 @@ Proof.
   inv H; rewrite H2; auto.
 Qed.
 
-Section System.
-  Variable sys: System.
-
-  Lemma internal_external_negb:
-    forall idx,
-      isInternal sys idx = negb (isExternal sys idx).
-  Proof.
-    unfold isInternal, isExternal; intros.
-    find_if_inside; auto.
-  Qed.
+Lemma ValidMsgsExtIn_merqsOf:
+  forall {MsgT SysT} `{HasMsg MsgT} `{IsSystem SysT}
+         (sys1: SysT) (eins: list (Id MsgT)),
+    ValidMsgsExtIn sys1 eins ->
+    forall sys2,
+      merqsOf sys1 = merqsOf sys2 ->
+      ValidMsgsExtIn sys2 eins.
+Proof.
+  unfold ValidMsgsExtIn; intros.
+  dest; split; auto.
+  rewrite <-H2; assumption.
+Qed.
   
-  Lemma internal_not_external:
-    forall idx,
-      isInternal sys idx = true -> isExternal sys idx = false.
-  Proof.
-    unfold isInternal, isExternal; intros.
-    find_if_inside; auto.
-  Qed.
-
-  Lemma external_not_internal:
-    forall idx,
-      isExternal sys idx = true -> isInternal sys idx = false.
-  Proof.
-    unfold isInternal, isExternal; intros.
-    find_if_inside; auto.
-  Qed.
-
-  Lemma internal_external_false:
-    forall idx,
-      isInternal sys idx = true -> isExternal sys idx = true -> False.
-  Proof.
-    unfold isInternal, isExternal; intros.
-    find_if_inside; intuition.
-  Qed.
-
-  Context {MsgT: Type} `{HasMsg MsgT}.
-
-  Lemma fromInternal_fromExternal_negb:
-    forall msg: MsgT,
-      fromInternal sys msg = negb (fromExternal sys msg).
-  Proof.
-    unfold fromInternal, fromExternal; intros.
-    apply internal_external_negb.
-  Qed.
-  
-  Lemma fromInternal_not_fromExternal:
-    forall msg: MsgT,
-      fromInternal sys msg = true -> fromExternal sys msg = false.
-  Proof.
-    unfold fromInternal, fromExternal; intros.
-    apply internal_not_external; auto.
-  Qed.
-
-  Lemma fromExternal_not_fromInternal:
-    forall msg: MsgT,
-      fromExternal sys msg = true -> fromInternal sys msg = false.
-  Proof.
-    unfold fromInternal, fromExternal; intros.
-    apply external_not_internal; auto.
-  Qed.
-
-  Lemma fromInternal_fromExternal_false:
-    forall msg: MsgT,
-      fromInternal sys msg = true -> fromExternal sys msg = true -> False.
-  Proof.
-    unfold fromInternal, fromExternal; intros.
-    eapply internal_external_false; eauto.
-  Qed.
-
-  Lemma toInternal_toExternal_negb:
-    forall msg: MsgT,
-      toInternal sys msg = negb (toExternal sys msg).
-  Proof.
-    unfold toInternal, toExternal; intros.
-    apply internal_external_negb.
-  Qed.
-  
-  Lemma toInternal_not_toExternal:
-    forall msg: MsgT,
-      toInternal sys msg = true -> toExternal sys msg = false.
-  Proof.
-    unfold toInternal, toExternal; intros.
-    apply internal_not_external; auto.
-  Qed.
-
-  Lemma toExternal_not_toInternal:
-    forall msg: MsgT,
-      toExternal sys msg = true -> toInternal sys msg = false.
-  Proof.
-    unfold toInternal, toExternal; intros.
-    apply external_not_internal; auto.
-  Qed.
-
-  Lemma toInternal_toExternal_false:
-    forall msg: MsgT,
-      toInternal sys msg = true -> toExternal sys msg = true -> False.
-  Proof.
-    unfold toInternal, toExternal; intros.
-    eapply internal_external_false; eauto.
-  Qed.
-
-  Lemma internal_extOuts_nil:
-    forall (mouts: list MsgT),
-      Forall (fun tmsg => toInternal sys tmsg = true) mouts ->
-      extOuts sys (map getMsg mouts) = nil.
-  Proof.
-    induction mouts; simpl; intros; [reflexivity|].
-    inv H0; unfold id, toExternal, maToExternal in *.
-    rewrite internal_not_external by assumption; auto.
-  Qed.
-
-  Lemma intOuts_Forall:
-    forall (msgs: list MsgT),
-      Forall (fun msg => toInternal sys msg = true) msgs ->
-      intOuts sys msgs = msgs.
-  Proof.
-    induction msgs; simpl; intros; [reflexivity|].
-    inv H0; rewrite H3.
-    rewrite IHmsgs by assumption.
-    reflexivity.
-  Qed.
-
-End System.
-
-Lemma extOuts_same_indicesOf:
-  forall (sys1 sys2: System) {MsgT} `{HasMsg MsgT} (msgs: list MsgT),
-    indicesOf sys1 = indicesOf sys2 ->
-    extOuts sys1 msgs = extOuts sys2 msgs.
+Lemma ValidMsgsExtOut_merssOf:
+  forall {MsgT SysT} `{HasMsg MsgT} `{IsSystem SysT}
+         (sys1: SysT) (eouts: list (Id MsgT)),
+    ValidMsgsExtOut sys1 eouts ->
+    forall sys2,
+      merssOf sys1 = merssOf sys2 ->
+      ValidMsgsExtOut sys2 eouts.
 Proof.
-  unfold_idx.
-  rewrite H0; reflexivity.
-Qed.
-
-Lemma intOuts_same_indicesOf:
-  forall (sys1 sys2: System) {MsgT} `{HasMsg MsgT} (msgs: list MsgT),
-    indicesOf sys1 = indicesOf sys2 ->
-    intOuts sys1 msgs = intOuts sys2 msgs.
-Proof.
-  unfold_idx.
-  rewrite H0; reflexivity.
-Qed.
-
-Lemma WellDistrMsgsIn_NoDup_msgAddrOf:
-  forall mins,
-    WellDistrMsgsIn mins ->
-    NoDup (map msgAddrOf mins).
-Proof.
-  intros; hnf in H.
-  induction mins; simpl; intros; [constructor|].
-  inv H.
-  constructor; auto.
-  intro Hx; elim H2.
-  destruct a as [[[from1 to1 chn1] tid1] val1]; cbn in *.
-  clear -Hx; induction mins; [elim Hx|].
-  inv Hx.
-  - destruct a as [[[from2 to2 chn2] tid2] val2]; cbn in *.
-    inv H; auto.
-  - right; auto.
-Qed.
-
-Lemma WellDistrMsgsOut_NoDup_msgAddrOf:
-  forall mouts,
-    WellDistrMsgsOut mouts ->
-    NoDup (map msgAddrOf mouts).
-Proof.
-  intros; hnf in H.
-  induction mouts; simpl; intros; [constructor|].
-  inv H.
-  constructor; auto.
-  intro Hx; elim H2.
-  destruct a as [[[from1 to1 chn1] tid1] val1]; cbn in *.
-  clear -Hx; induction mouts; [elim Hx|].
-  inv Hx.
-  - destruct a as [[[from2 to2 chn2] tid2] val2]; cbn in *.
-    inv H; auto.
-  - right; auto.
-Qed.
-
-Lemma ValidMsgsOut_ValidMsgsExtIn_DisjList:
-  forall oidx sys,
-    In oidx (sys_inds sys) ->
-    forall eins mouts,
-      ValidMsgsOut oidx mouts ->
-      ValidMsgsExtIn sys eins ->
-      DisjList (map msgAddrOf mouts) (map msgAddrOf eins).
-Proof.
-  intros.
-  destruct H0, H1.
-  clear H2 H3.
-
-  assert (forall ma, In ma (map msgAddrOf mouts) -> isInternal sys (ma_from ma) = true).
-  { intros.
-    clear -H H0 H2; induction mouts; [elim H2|].
-    inv H0; inv H2; auto.
-    dest; unfold isInternal.
-    destruct a as [[[from to chn] tid] val]; simpl; cbn in H0; subst.
-    destruct (_ ?<n _); auto.
-  }
-
-  assert (forall ma, In ma (map msgAddrOf eins) -> isInternal sys (ma_from ma) = false).
-  { intros.
-    clear -H1 H3; induction eins; [elim H3|].
-    inv H1; inv H3; auto.
-    dest.
-    unfold fromExternal in H.
-    destruct a as [[[from to chn] tid] val]; simpl; cbn in *.
-    apply external_not_internal; auto.
-  }
-
-  red; intros.
-  destruct (in_dec msgAddr_dec e (map msgAddrOf mouts)); auto.
-  destruct (in_dec msgAddr_dec e (map msgAddrOf eins)); auto.
-  exfalso; specialize (H2 _ i); specialize (H3 _ i0).
-  congruence.
-Qed.
-
-Lemma ValidMsgsIn_getMsg_eq_from_to:
-  forall {MsgT1} `{HasMsg MsgT1} oidx (mins1: list MsgT1),
-    Forall
-      (fun msg: MsgT1 => mid_to (msg_id (getMsg msg)) = oidx /\
-                         mid_from (msg_id (getMsg msg)) <> oidx) mins1 ->
-    forall {MsgT2} `{HasMsg MsgT2} (mins2: list MsgT2),
-      map getMsg mins1 = map getMsg mins2 ->
-      Forall
-        (fun msg: MsgT2 =>
-           mid_to (msg_id (getMsg msg)) = oidx /\
-           mid_from (msg_id (getMsg msg)) <> oidx) mins2.
-Proof.
-  induction mins1; simpl; intros.
-  - apply eq_sym, map_eq_nil in H2; subst.
-    constructor.
-  - destruct mins2 as [|b mins2]; [discriminate|].
-    simpl in H2; inv H2.
-    inv H0.
-    constructor; auto.
-    rewrite <-H4; auto.
-Qed.
-
-Lemma ValidMsgsIn_getMsg_eq_WellDistrMsgsIn:
-  forall {MsgT1} `{HasMsg MsgT1} (mins1: list MsgT1),
-    WellDistrMsgsIn mins1 ->
-    forall {MsgT2} `{HasMsg MsgT2} (mins2: list MsgT2),
-      map getMsg mins1 = map getMsg mins2 ->
-      WellDistrMsgsIn mins2.
-Proof.
-  unfold WellDistrMsgsIn; induction mins1; simpl; intros.
-  - apply eq_sym, map_eq_nil in H2; subst.
-    constructor.
-  - destruct mins2 as [|b mins2]; [discriminate|].
-    simpl in H2; inv H2.
-    inv H0.
-    simpl; constructor; auto.
-
-    assert (map (fun m: MsgT1 => (mid_from (msg_id (getMsg m)),
-                                  mid_chn (msg_id (getMsg m)))) mins1 =
-            map (fun m: MsgT2 => (mid_from (msg_id (getMsg m)),
-                                  mid_chn (msg_id (getMsg m)))) mins2).
-    { clear -H5.
-      generalize dependent mins2.
-      induction mins1; simpl; intros.
-      { apply eq_sym, map_eq_nil in H5; subst; auto. }
-      { destruct mins2 as [|b mins2]; [discriminate|].
-        simpl in H5; inv H5.
-        simpl.
-        erewrite IHmins1 by eassumption.
-        rewrite H2; reflexivity.
-      }
-    }
-    
-    rewrite <-H4, <-H0; assumption.
-Qed.
-
-Lemma ValidMsgsIn_getMsg_eq:
-  forall {MsgT1} `{HasMsg MsgT1} oidx (mins1: list MsgT1),
-    ValidMsgsIn oidx mins1 ->
-    forall {MsgT2} `{HasMsg MsgT2} (mins2: list MsgT2),
-      map getMsg mins1 = map getMsg mins2 ->
-      ValidMsgsIn oidx mins2.
-Proof.
-  intros; destruct H0; split.
-  - eapply ValidMsgsIn_getMsg_eq_from_to in H0; [|eassumption].
-    assumption.
-  - eapply ValidMsgsIn_getMsg_eq_WellDistrMsgsIn in H3; [|eassumption].
-    assumption.
-Qed.
-
-Lemma ValidMsgsExtIn_same_indices:
-  forall {SysT} `{IsSystem SysT} (impl1 impl2: SysT),
-    indicesOf impl1 = indicesOf impl2 ->
-    forall {MsgT} `{HasMsg MsgT} (eins: list MsgT),
-      ValidMsgsExtIn impl1 eins ->
-      ValidMsgsExtIn impl2 eins.
-Proof.
-  intros.
-  destruct H2; split; auto.
-  clear H3.
-  induction eins; simpl; [constructor|].
-  inv H2; dest.
-  constructor; auto.
-  split.
-  - unfold_idx.
-    rewrite <-H0; assumption.
-  - unfold_idx.
-    rewrite <-H0; assumption.
-Qed.    
-
-Lemma ValidMsgsExtOut_same_indices:
-  forall {SysT} `{IsSystem SysT} (impl1 impl2: SysT),
-    indicesOf impl1 = indicesOf impl2 ->
-    forall {MsgT} `{HasMsg MsgT} (eouts: list MsgT),
-      ValidMsgsExtOut impl1 eouts ->
-      ValidMsgsExtOut impl2 eouts.
-Proof.
-  intros.
-  destruct H2; split; auto.
-  clear H3.
-  induction eouts; simpl; [constructor|].
-  inv H2; dest.
-  constructor; auto.
-  split.
-  - unfold_idx.
-    rewrite <-H0; assumption.
-  - unfold_idx.
-    rewrite <-H0; assumption.
-Qed.
-
-Lemma ValidMsgsIn_MsgAddr_NoDup:
-  forall {MsgT} `{HasMsg MsgT} oidx (mins: list MsgT),
-    ValidMsgsIn oidx mins ->
-    NoDup (map (fun msg => mid_addr (msg_id (getMsg msg))) mins).
-Proof.
-  intros; destruct H0.
-  clear -H1; induction mins; [constructor|].
-  inv H1.
-  simpl; constructor; auto.
-  intro Hx; elim H3; clear -Hx.
-  induction mins; [elim Hx|].
-  simpl in *; destruct Hx; auto.
-  destruct (getMsg a0) as [[[from1 to1 chn1] tid1] val1].
-  destruct (getMsg a) as [[[from2 to2 chn2] tid2] val2].
-  cbn in *; inv H0.
-  auto.
-Qed.
-
-Lemma ValidMsgsOut_MsgAddr_NoDup:
-  forall {MsgT} `{HasMsg MsgT} oidx (mouts: list MsgT),
-    ValidMsgsOut oidx mouts ->
-    NoDup (map (fun msg => mid_addr (msg_id (getMsg msg))) mouts).
-Proof.
-  intros; destruct H0.
-  clear -H1; induction mouts; [constructor|].
-  inv H1.
-  simpl; constructor; auto.
-  intro Hx; elim H3; clear -Hx.
-  induction mouts; [elim Hx|].
-  simpl in *; destruct Hx; auto.
-  destruct (getMsg a0) as [[[from1 to1 chn1] tid1] val1].
-  destruct (getMsg a) as [[[from2 to2 chn2] tid2] val2].
-  cbn in *; inv H0.
-  auto.
-Qed.
-
-Lemma MsgAddr_NoDup_toTMsg:
-  forall (msgs: list Msg),
-    NoDup (map (fun msg => mid_addr (msg_id (getMsg msg))) msgs) ->
-    forall ti,
-      NoDup (map (fun msg => mid_addr (msg_id (getMsg msg))) (toTMsgs ti msgs)).
-Proof.
-  induction msgs; simpl; intros; [constructor|].
-  inv H.
-  constructor; auto.
-  intro Hx; elim H2; clear -Hx.
-  induction msgs; [elim Hx|].
-  simpl in *; destruct Hx; auto.
-Qed.
-
-Lemma idx_in_sys_internal:
-  forall oidx {SysT} `{IsSystem SysT} (sys: SysT),
-    In oidx (indicesOf sys) ->
-    isInternal sys oidx = true.
-Proof.
-  unfold isInternal; intros.
-  find_if_inside; auto.
-Qed.
-
-Lemma step_t_int_internal:
-  forall sys st1 orule ins outs st2,
-    step_t sys st1 (RlblInt orule ins outs) st2 ->
-    Forall (fun msg => toInternal sys msg = true) ins.
-Proof.
-  intros; inv H; [constructor|].
-  clear -H4 H8.
-  induction ins; [constructor|].
-  assert (ValidMsgsIn (rule_oidx rule) ins)
-    by (destruct H8; inv H; inv H0; split; auto).
-  constructor; auto.
-  destruct H8; inv H0; dest; subst.
-  rewrite <-H0 in H4.
-  apply idx_in_sys_internal; auto.
+  unfold ValidMsgsExtOut; intros.
+  dest; split; auto.
+  rewrite <-H2; assumption.
 Qed.
 
 Lemma step_t_tid_next:
   forall sys st1 orule ins outs ts st2,
     step_t sys st1 (RlblInt orule ins outs) st2 ->
     outs <> nil ->
-    Forall (fun tmsg => tmsg_info tmsg = None) ins ->
+    Forall (fun tmsg => tmsg_info tmsg = None) (valsOf ins) ->
     Forall (fun tmsg => match tmsg_info tmsg with
                         | Some ti => tinfo_tid ti = ts
                         | None => True
-                        end) outs ->
+                        end) (valsOf outs) ->
     tst_tid st2 = ts.
 Proof.
   intros.
@@ -563,74 +150,6 @@ Theorem step_t_sound:
         tToMLabel tlbl = lbl /\
         TStateRel ntst nst.
 Proof.
-  intros.
-  destruct ptst as [poss porqs pmsgs ptid].
-  destruct H0 as [? [? ?]]; simpl in *.
-  inv H.
-  - do 2 eexists; repeat econstructor; eauto.
-  - eexists; exists (RlblIns (toTMsgsU eins)).
-    split; [|split].
-    + econstructor; eauto.
-    + simpl; f_equal.
-      clear; induction eins; auto.
-      simpl; rewrite IHeins; reflexivity.
-    + repeat split; simpl; auto.
-      red in H2; simpl in H2; subst.
-      clear; red.
-      unfold distributeMsgs; simpl.
-      rewrite map_app.
-      f_equal.
-      clear; induction eins; auto.
-      simpl; rewrite IHeins; reflexivity.
-  - admit.
-  - red in H2; simpl in H2; subst.
-    red in H1; simpl in H1.
-
-    assert (exists tmsgs,
-               map tmsg_msg tmsgs = ins /\
-               Forall (FirstMP pmsgs) tmsgs).
-    { admit. }
-    destruct H as [tmsgs [? ?]]; subst.
-
-    eexists.
-    eexists (RlblInt (Some rule) _ _).
-    split; [|split].
-    + remember (porqs @[rule_oidx rule]) as oorq.
-      destruct oorq as [orq|];
-        [|specialize (H1 (rule_oidx rule));
-          rewrite <-Heqoorq, H6 in H1; exfalso; auto].
-      apply eq_sym in Heqoorq.
-
-      econstructor; try reflexivity; try eassumption.
-      * auto.
-      * eapply ValidMsgsIn_getMsg_eq
-          with (mins1:= map tmsg_msg tmsgs); [assumption|].
-        clear; induction tmsgs; auto.
-        simpl in *.
-        rewrite IHtmsgs; reflexivity.
-      * rewrite <-H9.
-        clear; induction tmsgs; simpl; auto.
-        rewrite IHtmsgs; reflexivity.
-      * specialize (H1 (rule_oidx rule)).
-        rewrite Heqoorq, H6 in H1; subst.
-        assumption.
-      * instantiate (2:= pos).
-        admit.
-    + clear.
-      cbn; f_equal.
-      induction iouts; simpl; auto.
-      rewrite IHiouts; reflexivity.
-    + split; [|split]; simpl; auto.
-      * admit.
-      * red; unfold distributeMsgs.
-        rewrite map_app; f_equal.
-        { apply mmap_removeMsgs.
-          intros; reflexivity.
-        }
-        { clear; induction iouts; simpl; auto.
-          rewrite IHiouts; reflexivity.
-        }
-        
 Admitted.
 
 Lemma steps_split:
@@ -687,7 +206,7 @@ Qed.
 Lemma behaviorOf_preserved:
   forall {SysT1 SysT2} `{IsSystem SysT1} `{IsSystem SysT2}
          (impl1: SysT1) (impl2: SysT2),
-    indicesOf impl1 = indicesOf impl2 ->
+    oindsOf impl1 = oindsOf impl2 ->
     forall hst,
       behaviorOf impl1 hst = behaviorOf impl2 hst.
 Proof.
@@ -697,23 +216,21 @@ Qed.
 
 Theorem refines_refl:
   forall {SysT StateT LabelT} `{IsSystem SysT} `{HasInit SysT StateT} `{HasLabel LabelT}
-         (ss: Steps SysT StateT LabelT) sys, ss # ss |-- sys ⊑[id] sys.
+         (ss: Steps SysT StateT LabelT) sys, ss # ss |-- sys ⊑ sys.
 Proof.
   unfold Refines; intros.
-  rewrite map_id.
   assumption.
 Qed.
 
 Theorem refines_trans:
   forall {SysT StateT LabelT} `{IsSystem SysT} `{HasInit SysT StateT} `{HasLabel LabelT}
-         (ss1 ss2 ss3: Steps SysT StateT LabelT) p q s1 s2 s3,
-    ss1 # ss2 |-- s1 ⊑[p] s2 ->
-    ss2 # ss3 |-- s2 ⊑[q] s3 ->
-    ss1 # ss3 |-- s1 ⊑[fun l => q (p l)] s3.
+         (ss1 ss2 ss3: Steps SysT StateT LabelT) s1 s2 s3,
+    ss1 # ss2 |-- s1 ⊑ s2 ->
+    ss2 # ss3 |-- s2 ⊑ s3 ->
+    ss1 # ss3 |-- s1 ⊑ s3.
 Proof.
   unfold Refines; intros.
   specialize (H3 _ (H2 _ H4)).
-  rewrite map_trans in H3.
   assumption.
 Qed.
 
