src/Serial.v
@@ -13,20 +13,21 @@ Section PerSystem.
    *    and all [hdl]s have the same [tinfo_tid]. It means that the history is
    *    for a single transaction.
    *)
-  Inductive Atomic: TrsId -> Msg -> THistory -> MessagePool TMsg -> Prop :=
+  Inductive Atomic: TrsId -> Id Msg -> THistory -> MessagePool TMsg -> Prop :=
   | AtomicStart:
       forall ts rqr rq houts,
-        fromExternal sys rq = true ->
-        ForallMP (fun tmsg => tmsg_info tmsg =
-                              Some (buildTInfo ts (rq :: nil))) houts ->
-        Atomic ts rq (RlblInt (Some rqr) (toTMsgU rq :: nil) houts :: nil) houts
+        In (idOf rq) (merqsOf sys) ->
+        Forall (fun idm => tmsg_info (valOf idm) =
+                           Some (buildTInfo ts (rq :: nil))) houts ->
+        Atomic ts rq (RlblInt (Some rqr) (liftI toTMsgU rq :: nil) houts :: nil)
+               (enqMsgs houts (emptyMP _))
   | AtomicCont:
       forall ts rq hst rule msgs mouts houts,
         Atomic ts rq hst mouts ->
         msgs <> nil ->
-        SubList msgs mouts ->
+        Forall (fun idm => InMP (idOf idm) (valOf idm) mouts) msgs ->
         Atomic ts rq (RlblInt (Some rule) msgs houts :: hst)
-               (distributeMsgs houts (removeMsgs msgs mouts)).
+               (enqMsgs houts (deqMsgs (idsOf msgs) mouts)).
 
   Inductive Transactional: THistory -> Prop :=
   | TrsSlt:
@@ -50,15 +51,6 @@ Section PerSystem.
       hst = List.concat trss.
 
 End PerSystem.
-
-(** Transaction messages in [MessagePool] *)
-
-Definition trsMessages (trsInfo: TInfo) (mp: MessagePool TMsg) : list TMsg :=
-  filter (fun tmsg =>
-            match tmsg_info tmsg with
-            | Some tinfo => if tinfo_dec tinfo trsInfo then true else false
-            | None => false
-            end) mp.
 
 (** Serializability *)
 
